Risc0/Gadgets/ComputeDecode/Witness/WeakestPresPart13.lean
@@ -11,44 +11,41 @@ open MLIRNotation
 def part13_state (st: State) : State :=
   
           (State.set!
-              (State.set! st { name := "data" } 4 (Option.get! st.felts[({ name := "%92" }: FeltVar)]!)[felts][{ name := "%93" }] ←
-                ↑(Bitvec.toNat
-                    (Bitvec.and (Bitvec.ofNat 256 (ZMod.val (Option.get! (State.felts st { name := "%22" }))))
-                      (Bitvec.ofNat 256 (ZMod.val (Option.get! (State.felts st { name := "%4" })))))))
-              { name := "data" } 3
-              ↑(Bitvec.toNat
-                  (Bitvec.and (Bitvec.ofNat 256 (ZMod.val (Option.get! (State.felts st { name := "%22" }))))
-                    (Bitvec.ofNat 256
-                      (ZMod.val (Option.get! (State.felts st { name := "%4" }))))))[felts][{ name := "%94" }] ←
-            ↑(Bitvec.toNat
-                (Bitvec.and (Bitvec.ofNat 256 (ZMod.val (Option.get! (State.felts st { name := "%21" }))))
-                  (Bitvec.ofNat 256
-                    (ZMod.val
-                      (Option.get!
-                        (State.felts st
-                          {
-                            name :=
-                              "%19" }))))))) 
+            (((st[felts][{ name := "%96" }] ←
+                  feltBitAnd (Option.get! (State.felts st { name := "%21" }))
+                    (Option.get! (State.felts st { name := "%3" })))[felts][{ name := "%2" }] ←
+                1981808641)[felts][{ name := "%97" }] ←
+              feltBitAnd (Option.get! (State.felts st { name := "%21" }))
+                  (Option.get! (State.felts st { name := "%3" })) *
+                1981808641)
+            { name := "data" } 15
+            (feltBitAnd (Option.get! (State.felts st { name := "%21" }))
+                (Option.get! (State.felts st { name := "%3" })) *
+              1981808641)) 
+
+def part13_drops (st: State) : State :=
+  State.dropFelts (State.dropFelts (State.dropFelts (st) ⟨"%96"⟩) ⟨"%2"⟩) ⟨"%97"⟩
 
 -- Run the program from part13 onwards by using part13_state rather than Code.part13
 def part13_state_update (st: State): State :=
-  Γ (part13_state st) ⟦Code.part14; Code.part15; Code.part16; Code.part17; Code.part18; Code.part19; Code.part20; Code.part21; Code.part22; Code.part23; Code.part24; Code.part25; Code.part26; Code.part27; Code.part28; Code.part29; Code.part30; Code.part31⟧
+  Γ (part13_drops (part13_state st)) ⟦Code.part14;dropfelt ⟨"%14"⟩;dropfelt ⟨"%1"⟩;dropfelt ⟨"%98"⟩;dropfelt ⟨"%99"⟩;Code.part15;dropfelt ⟨"%6"⟩;dropfelt ⟨"%5"⟩;dropfelt ⟨"%4"⟩;dropfelt ⟨"%100"⟩;dropfelt ⟨"%101"⟩;Code.part16;dropfelt ⟨"%18"⟩;dropfelt ⟨"%102"⟩;dropfelt ⟨"%103"⟩;Code.part17;dropfelt ⟨"%104"⟩;dropfelt ⟨"%0"⟩;dropfelt ⟨"%105"⟩;Code.part18;dropfelt ⟨"%26"⟩;Code.part19;dropfelt ⟨"%28"⟩;dropfelt ⟨"%29"⟩;dropfelt ⟨"%30"⟩;dropfelt ⟨"%31"⟩;Code.part20;dropfelt ⟨"%27"⟩;dropfelt ⟨"%32"⟩;dropfelt ⟨"%33"⟩;dropfelt ⟨"%25"⟩;Code.part21;dropfelt ⟨"%3"⟩;dropfelt ⟨"%34"⟩;dropfelt ⟨"%35"⟩;dropfelt ⟨"%36"⟩;dropfelt ⟨"%37"⟩;Code.part22;dropfelt ⟨"%23"⟩;dropfelt ⟨"%38"⟩;dropfelt ⟨"%24"⟩;dropfelt ⟨"%39"⟩;dropfelt ⟨"%40"⟩;Code.part23;dropfelt ⟨"%11"⟩;dropfelt ⟨"%42"⟩;dropfelt ⟨"%45"⟩;Code.part24;dropfelt ⟨"%13"⟩;dropfelt ⟨"%46"⟩;dropfelt ⟨"%47"⟩;dropfelt ⟨"%48"⟩;Code.part25;dropfelt ⟨"%43"⟩;dropfelt ⟨"%49"⟩;dropfelt ⟨"%44"⟩;dropfelt ⟨"%50"⟩;dropfelt ⟨"%51"⟩;Code.part26;dropfelt ⟨"%22"⟩;dropfelt ⟨"%52"⟩;dropfelt ⟨"%41"⟩;dropfelt ⟨"%53"⟩;dropfelt ⟨"%54"⟩;Code.part27;dropfelt ⟨"%7"⟩;dropfelt ⟨"%56"⟩;dropfelt ⟨"%59"⟩;Code.part28;dropfelt ⟨"%15"⟩;dropfelt ⟨"%60"⟩;dropfelt ⟨"%58"⟩;dropfelt ⟨"%61"⟩;dropfelt ⟨"%63"⟩;Code.part29;dropfelt ⟨"%57"⟩;dropfelt ⟨"%62"⟩;dropfelt ⟨"%64"⟩;dropfelt ⟨"%65"⟩;dropfelt ⟨"%66"⟩;dropfelt ⟨"%55"⟩;Code.part30;dropfelt ⟨"%19"⟩;dropfelt ⟨"%21"⟩;dropfelt ⟨"%67"⟩;dropfelt ⟨"%68"⟩;dropfelt ⟨"%70"⟩;Code.part31;dropfelt ⟨"%20"⟩;dropfelt ⟨"%71"⟩;dropfelt ⟨"%69"⟩;dropfelt ⟨"%72"⟩;dropfelt ⟨"%73"⟩⟧
 
 -- Prove that substituting part13_state for Code.part13 produces the same result
 lemma part13_wp {st : State} {y0 y1 y2 y3 y4 y5 y6 y7 y8 y9 y10 y11 y12 y13 y14 y15 y16 y17 : Option Felt} :
-  Code.getReturn (MLIR.runProgram (Code.part13; Code.part14; Code.part15; Code.part16; Code.part17; Code.part18; Code.part19; Code.part20; Code.part21; Code.part22; Code.part23; Code.part24; Code.part25; Code.part26; Code.part27; Code.part28; Code.part29; Code.part30; Code.part31) st) = [y0, y1, y2, y3, y4, y5, y6, y7, y8, y9, y10, y11, y12, y13, y14, y15, y16, y17] ↔
+  Code.getReturn (MLIR.runProgram (Code.part13;dropfelt ⟨"%96"⟩;dropfelt ⟨"%2"⟩;dropfelt ⟨"%97"⟩;Code.part14;dropfelt ⟨"%14"⟩;dropfelt ⟨"%1"⟩;dropfelt ⟨"%98"⟩;dropfelt ⟨"%99"⟩;Code.part15;dropfelt ⟨"%6"⟩;dropfelt ⟨"%5"⟩;dropfelt ⟨"%4"⟩;dropfelt ⟨"%100"⟩;dropfelt ⟨"%101"⟩;Code.part16;dropfelt ⟨"%18"⟩;dropfelt ⟨"%102"⟩;dropfelt ⟨"%103"⟩;Code.part17;dropfelt ⟨"%104"⟩;dropfelt ⟨"%0"⟩;dropfelt ⟨"%105"⟩;Code.part18;dropfelt ⟨"%26"⟩;Code.part19;dropfelt ⟨"%28"⟩;dropfelt ⟨"%29"⟩;dropfelt ⟨"%30"⟩;dropfelt ⟨"%31"⟩;Code.part20;dropfelt ⟨"%27"⟩;dropfelt ⟨"%32"⟩;dropfelt ⟨"%33"⟩;dropfelt ⟨"%25"⟩;Code.part21;dropfelt ⟨"%3"⟩;dropfelt ⟨"%34"⟩;dropfelt ⟨"%35"⟩;dropfelt ⟨"%36"⟩;dropfelt ⟨"%37"⟩;Code.part22;dropfelt ⟨"%23"⟩;dropfelt ⟨"%38"⟩;dropfelt ⟨"%24"⟩;dropfelt ⟨"%39"⟩;dropfelt ⟨"%40"⟩;Code.part23;dropfelt ⟨"%11"⟩;dropfelt ⟨"%42"⟩;dropfelt ⟨"%45"⟩;Code.part24;dropfelt ⟨"%13"⟩;dropfelt ⟨"%46"⟩;dropfelt ⟨"%47"⟩;dropfelt ⟨"%48"⟩;Code.part25;dropfelt ⟨"%43"⟩;dropfelt ⟨"%49"⟩;dropfelt ⟨"%44"⟩;dropfelt ⟨"%50"⟩;dropfelt ⟨"%51"⟩;Code.part26;dropfelt ⟨"%22"⟩;dropfelt ⟨"%52"⟩;dropfelt ⟨"%41"⟩;dropfelt ⟨"%53"⟩;dropfelt ⟨"%54"⟩;Code.part27;dropfelt ⟨"%7"⟩;dropfelt ⟨"%56"⟩;dropfelt ⟨"%59"⟩;Code.part28;dropfelt ⟨"%15"⟩;dropfelt ⟨"%60"⟩;dropfelt ⟨"%58"⟩;dropfelt ⟨"%61"⟩;dropfelt ⟨"%63"⟩;Code.part29;dropfelt ⟨"%57"⟩;dropfelt ⟨"%62"⟩;dropfelt ⟨"%64"⟩;dropfelt ⟨"%65"⟩;dropfelt ⟨"%66"⟩;dropfelt ⟨"%55"⟩;Code.part30;dropfelt ⟨"%19"⟩;dropfelt ⟨"%21"⟩;dropfelt ⟨"%67"⟩;dropfelt ⟨"%68"⟩;dropfelt ⟨"%70"⟩;Code.part31;dropfelt ⟨"%20"⟩;dropfelt ⟨"%71"⟩;dropfelt ⟨"%69"⟩;dropfelt ⟨"%72"⟩;dropfelt ⟨"%73"⟩) st) = [y0, y1, y2, y3, y4, y5, y6, y7, y8, y9, y10, y11, y12, y13, y14, y15, y16, y17] ↔
   Code.getReturn (part13_state_update st) = [y0, y1, y2, y3, y4, y5, y6, y7, y8, y9, y10, y11, y12, y13, y14, y15, y16, y17] := by
   unfold MLIR.runProgram; simp only
-  generalize eq : (Code.part14; Code.part15; Code.part16; Code.part17; Code.part18; Code.part19; Code.part20; Code.part21; Code.part22; Code.part23; Code.part24; Code.part25; Code.part26; Code.part27; Code.part28; Code.part29; Code.part30; Code.part31) = prog
+  generalize eq : (dropfelt ⟨"%96"⟩;dropfelt ⟨"%2"⟩;dropfelt ⟨"%97"⟩;Code.part14;dropfelt ⟨"%14"⟩;dropfelt ⟨"%1"⟩;dropfelt ⟨"%98"⟩;dropfelt ⟨"%99"⟩;Code.part15;dropfelt ⟨"%6"⟩;dropfelt ⟨"%5"⟩;dropfelt ⟨"%4"⟩;dropfelt ⟨"%100"⟩;dropfelt ⟨"%101"⟩;Code.part16;dropfelt ⟨"%18"⟩;dropfelt ⟨"%102"⟩;dropfelt ⟨"%103"⟩;Code.part17;dropfelt ⟨"%104"⟩;dropfelt ⟨"%0"⟩;dropfelt ⟨"%105"⟩;Code.part18;dropfelt ⟨"%26"⟩;Code.part19;dropfelt ⟨"%28"⟩;dropfelt ⟨"%29"⟩;dropfelt ⟨"%30"⟩;dropfelt ⟨"%31"⟩;Code.part20;dropfelt ⟨"%27"⟩;dropfelt ⟨"%32"⟩;dropfelt ⟨"%33"⟩;dropfelt ⟨"%25"⟩;Code.part21;dropfelt ⟨"%3"⟩;dropfelt ⟨"%34"⟩;dropfelt ⟨"%35"⟩;dropfelt ⟨"%36"⟩;dropfelt ⟨"%37"⟩;Code.part22;dropfelt ⟨"%23"⟩;dropfelt ⟨"%38"⟩;dropfelt ⟨"%24"⟩;dropfelt ⟨"%39"⟩;dropfelt ⟨"%40"⟩;Code.part23;dropfelt ⟨"%11"⟩;dropfelt ⟨"%42"⟩;dropfelt ⟨"%45"⟩;Code.part24;dropfelt ⟨"%13"⟩;dropfelt ⟨"%46"⟩;dropfelt ⟨"%47"⟩;dropfelt ⟨"%48"⟩;Code.part25;dropfelt ⟨"%43"⟩;dropfelt ⟨"%49"⟩;dropfelt ⟨"%44"⟩;dropfelt ⟨"%50"⟩;dropfelt ⟨"%51"⟩;Code.part26;dropfelt ⟨"%22"⟩;dropfelt ⟨"%52"⟩;dropfelt ⟨"%41"⟩;dropfelt ⟨"%53"⟩;dropfelt ⟨"%54"⟩;Code.part27;dropfelt ⟨"%7"⟩;dropfelt ⟨"%56"⟩;dropfelt ⟨"%59"⟩;Code.part28;dropfelt ⟨"%15"⟩;dropfelt ⟨"%60"⟩;dropfelt ⟨"%58"⟩;dropfelt ⟨"%61"⟩;dropfelt ⟨"%63"⟩;Code.part29;dropfelt ⟨"%57"⟩;dropfelt ⟨"%62"⟩;dropfelt ⟨"%64"⟩;dropfelt ⟨"%65"⟩;dropfelt ⟨"%66"⟩;dropfelt ⟨"%55"⟩;Code.part30;dropfelt ⟨"%19"⟩;dropfelt ⟨"%21"⟩;dropfelt ⟨"%67"⟩;dropfelt ⟨"%68"⟩;dropfelt ⟨"%70"⟩;Code.part31;dropfelt ⟨"%20"⟩;dropfelt ⟨"%71"⟩;dropfelt ⟨"%69"⟩;dropfelt ⟨"%72"⟩;dropfelt ⟨"%73"⟩) = prog
   unfold Code.part13
   MLIR
   rewrite [←eq]
-  unfold part13_state_update part13_state
+  rewrite [MLIR.run_seq_def,MLIR.run_dropfelt, MLIR.run_seq_def,MLIR.run_dropfelt, MLIR.run_seq_def,MLIR.run_dropfelt]
+  unfold part13_state_update part13_drops part13_state
   rfl
 
 lemma part13_updates_opaque {st : State} : 
   Code.getReturn (part12_state_update st) = [y0, y1, y2, y3, y4, y5, y6, y7, y8, y9, y10, y11, y12, y13, y14, y15, y16, y17] ↔
-  Code.getReturn (part13_state_update (part12_state st)) = [y0, y1, y2, y3, y4, y5, y6, y7, y8, y9, y10, y11, y12, y13, y14, y15, y16, y17] := by
+  Code.getReturn (part13_state_update (part12_drops (part12_state st))) = [y0, y1, y2, y3, y4, y5, y6, y7, y8, y9, y10, y11, y12, y13, y14, y15, y16, y17] := by
   simp [part12_state_update, part13_wp]
 
 end Risc0.ComputeDecode.Witness.WP
