Risc0/Gadgets/ComputeDecode/Witness/WeakestPresPart18.lean
@@ -9,58 +9,37 @@ open MLIRNotation
 
 -- The state obtained by running Code.part18 on st
 def part18_state (st: State) : State :=
-  (((State.set!
-              (st[felts][{ name := "%105" }] ←
-                ↑(Bitvec.toNat
-                    (Bitvec.and (Bitvec.ofNat 256 (ZMod.val (Option.get! (State.felts st { name := "%20" }))))
-                      (Bitvec.ofNat 256 (ZMod.val (Option.get! (State.felts st { name := "%0" })))))))
-              { name := "data" } 17
-              ↑(Bitvec.toNat
-                  (Bitvec.and (Bitvec.ofNat 256 (ZMod.val (Option.get! (State.felts st { name := "%20" }))))
-                    (Bitvec.ofNat 256 (ZMod.val (Option.get! (State.felts st { name := "%0" })))))))["%24"] ←ₛ
-            getImpl
-              (State.set!
-                (st[felts][{ name := "%105" }] ←
-                  ↑(Bitvec.toNat
-                      (Bitvec.and (Bitvec.ofNat 256 (ZMod.val (Option.get! (State.felts st { name := "%20" }))))
-                        (Bitvec.ofNat 256 (ZMod.val (Option.get! (State.felts st { name := "%0" })))))))
-                { name := "data" } 17
-                ↑(Bitvec.toNat
-                    (Bitvec.and (Bitvec.ofNat 256 (ZMod.val (Option.get! (State.felts st { name := "%20" }))))
-                      (Bitvec.ofNat 256 (ZMod.val (Option.get! (State.felts st { name := "%0" })))))))
-              { name := "data" } 0 13)["%25"] ←ₛ
-          getImpl
-            (State.set!
-              (st[felts][{ name := "%105" }] ←
-                ↑(Bitvec.toNat
-                    (Bitvec.and (Bitvec.ofNat 256 (ZMod.val (Option.get! (State.felts st { name := "%20" }))))
-                      (Bitvec.ofNat 256 (ZMod.val (Option.get! (State.felts st { name := "%0" })))))))
-              { name := "data" } 17
-              ↑(Bitvec.toNat
-                  (Bitvec.and (Bitvec.ofNat 256 (ZMod.val (Option.get! (State.felts st { name := "%20" }))))
-                    (Bitvec.ofNat 256 (ZMod.val (Option.get! (State.felts st { name := "%0" })))))))
-            { name := "data" } 0
-            0)
+  
+          ((((st[felts][{ name := "%7" }] ← 4)["%26"] ←ₛ getImpl st { name := "data" } 0 8)[felts][{ name := "%27" }] ←
+              Option.get!
+                  (State.felts ((st[felts][{ name := "%7" }] ← 4)["%26"] ←ₛ getImpl st { name := "data" } 0 8)
+                    { name := "%26" }) *
+                4)["%28"] ←ₛ
+            getImpl (st[felts][{ name := "%7" }] ← 4) { name := "data" } 0 9) 
+
+def part18_drops (st: State) : State :=
+  State.dropFelts (st) ⟨"%26"⟩
 
 -- Run the program from part18 onwards by using part18_state rather than Code.part18
 def part18_state_update (st: State): State :=
-  Γ (part18_state st) ⟦Code.part19; Code.part20; Code.part21; Code.part22; Code.part23; Code.part24; Code.part25; Code.part26; Code.part27; Code.part28; Code.part29; Code.part30; Code.part31⟧
+  Γ (part18_drops (part18_state st)) ⟦Code.part19;dropfelt ⟨"%28"⟩;dropfelt ⟨"%29"⟩;dropfelt ⟨"%30"⟩;dropfelt ⟨"%31"⟩;Code.part20;dropfelt ⟨"%27"⟩;dropfelt ⟨"%32"⟩;dropfelt ⟨"%33"⟩;dropfelt ⟨"%25"⟩;Code.part21;dropfelt ⟨"%3"⟩;dropfelt ⟨"%34"⟩;dropfelt ⟨"%35"⟩;dropfelt ⟨"%36"⟩;dropfelt ⟨"%37"⟩;Code.part22;dropfelt ⟨"%23"⟩;dropfelt ⟨"%38"⟩;dropfelt ⟨"%24"⟩;dropfelt ⟨"%39"⟩;dropfelt ⟨"%40"⟩;Code.part23;dropfelt ⟨"%11"⟩;dropfelt ⟨"%42"⟩;dropfelt ⟨"%45"⟩;Code.part24;dropfelt ⟨"%13"⟩;dropfelt ⟨"%46"⟩;dropfelt ⟨"%47"⟩;dropfelt ⟨"%48"⟩;Code.part25;dropfelt ⟨"%43"⟩;dropfelt ⟨"%49"⟩;dropfelt ⟨"%44"⟩;dropfelt ⟨"%50"⟩;dropfelt ⟨"%51"⟩;Code.part26;dropfelt ⟨"%22"⟩;dropfelt ⟨"%52"⟩;dropfelt ⟨"%41"⟩;dropfelt ⟨"%53"⟩;dropfelt ⟨"%54"⟩;Code.part27;dropfelt ⟨"%7"⟩;dropfelt ⟨"%56"⟩;dropfelt ⟨"%59"⟩;Code.part28;dropfelt ⟨"%15"⟩;dropfelt ⟨"%60"⟩;dropfelt ⟨"%58"⟩;dropfelt ⟨"%61"⟩;dropfelt ⟨"%63"⟩;Code.part29;dropfelt ⟨"%57"⟩;dropfelt ⟨"%62"⟩;dropfelt ⟨"%64"⟩;dropfelt ⟨"%65"⟩;dropfelt ⟨"%66"⟩;dropfelt ⟨"%55"⟩;Code.part30;dropfelt ⟨"%19"⟩;dropfelt ⟨"%21"⟩;dropfelt ⟨"%67"⟩;dropfelt ⟨"%68"⟩;dropfelt ⟨"%70"⟩;Code.part31;dropfelt ⟨"%20"⟩;dropfelt ⟨"%71"⟩;dropfelt ⟨"%69"⟩;dropfelt ⟨"%72"⟩;dropfelt ⟨"%73"⟩⟧
 
 -- Prove that substituting part18_state for Code.part18 produces the same result
 lemma part18_wp {st : State} {y0 y1 y2 y3 y4 y5 y6 y7 y8 y9 y10 y11 y12 y13 y14 y15 y16 y17 : Option Felt} :
-  Code.getReturn (MLIR.runProgram (Code.part18; Code.part19; Code.part20; Code.part21; Code.part22; Code.part23; Code.part24; Code.part25; Code.part26; Code.part27; Code.part28; Code.part29; Code.part30; Code.part31) st) = [y0, y1, y2, y3, y4, y5, y6, y7, y8, y9, y10, y11, y12, y13, y14, y15, y16, y17] ↔
+  Code.getReturn (MLIR.runProgram (Code.part18;dropfelt ⟨"%26"⟩;Code.part19;dropfelt ⟨"%28"⟩;dropfelt ⟨"%29"⟩;dropfelt ⟨"%30"⟩;dropfelt ⟨"%31"⟩;Code.part20;dropfelt ⟨"%27"⟩;dropfelt ⟨"%32"⟩;dropfelt ⟨"%33"⟩;dropfelt ⟨"%25"⟩;Code.part21;dropfelt ⟨"%3"⟩;dropfelt ⟨"%34"⟩;dropfelt ⟨"%35"⟩;dropfelt ⟨"%36"⟩;dropfelt ⟨"%37"⟩;Code.part22;dropfelt ⟨"%23"⟩;dropfelt ⟨"%38"⟩;dropfelt ⟨"%24"⟩;dropfelt ⟨"%39"⟩;dropfelt ⟨"%40"⟩;Code.part23;dropfelt ⟨"%11"⟩;dropfelt ⟨"%42"⟩;dropfelt ⟨"%45"⟩;Code.part24;dropfelt ⟨"%13"⟩;dropfelt ⟨"%46"⟩;dropfelt ⟨"%47"⟩;dropfelt ⟨"%48"⟩;Code.part25;dropfelt ⟨"%43"⟩;dropfelt ⟨"%49"⟩;dropfelt ⟨"%44"⟩;dropfelt ⟨"%50"⟩;dropfelt ⟨"%51"⟩;Code.part26;dropfelt ⟨"%22"⟩;dropfelt ⟨"%52"⟩;dropfelt ⟨"%41"⟩;dropfelt ⟨"%53"⟩;dropfelt ⟨"%54"⟩;Code.part27;dropfelt ⟨"%7"⟩;dropfelt ⟨"%56"⟩;dropfelt ⟨"%59"⟩;Code.part28;dropfelt ⟨"%15"⟩;dropfelt ⟨"%60"⟩;dropfelt ⟨"%58"⟩;dropfelt ⟨"%61"⟩;dropfelt ⟨"%63"⟩;Code.part29;dropfelt ⟨"%57"⟩;dropfelt ⟨"%62"⟩;dropfelt ⟨"%64"⟩;dropfelt ⟨"%65"⟩;dropfelt ⟨"%66"⟩;dropfelt ⟨"%55"⟩;Code.part30;dropfelt ⟨"%19"⟩;dropfelt ⟨"%21"⟩;dropfelt ⟨"%67"⟩;dropfelt ⟨"%68"⟩;dropfelt ⟨"%70"⟩;Code.part31;dropfelt ⟨"%20"⟩;dropfelt ⟨"%71"⟩;dropfelt ⟨"%69"⟩;dropfelt ⟨"%72"⟩;dropfelt ⟨"%73"⟩) st) = [y0, y1, y2, y3, y4, y5, y6, y7, y8, y9, y10, y11, y12, y13, y14, y15, y16, y17] ↔
   Code.getReturn (part18_state_update st) = [y0, y1, y2, y3, y4, y5, y6, y7, y8, y9, y10, y11, y12, y13, y14, y15, y16, y17] := by
   unfold MLIR.runProgram; simp only
-  generalize eq : (Code.part19; Code.part20; Code.part21; Code.part22; Code.part23; Code.part24; Code.part25; Code.part26; Code.part27; Code.part28; Code.part29; Code.part30; Code.part31) = prog
+  generalize eq : (dropfelt ⟨"%26"⟩;Code.part19;dropfelt ⟨"%28"⟩;dropfelt ⟨"%29"⟩;dropfelt ⟨"%30"⟩;dropfelt ⟨"%31"⟩;Code.part20;dropfelt ⟨"%27"⟩;dropfelt ⟨"%32"⟩;dropfelt ⟨"%33"⟩;dropfelt ⟨"%25"⟩;Code.part21;dropfelt ⟨"%3"⟩;dropfelt ⟨"%34"⟩;dropfelt ⟨"%35"⟩;dropfelt ⟨"%36"⟩;dropfelt ⟨"%37"⟩;Code.part22;dropfelt ⟨"%23"⟩;dropfelt ⟨"%38"⟩;dropfelt ⟨"%24"⟩;dropfelt ⟨"%39"⟩;dropfelt ⟨"%40"⟩;Code.part23;dropfelt ⟨"%11"⟩;dropfelt ⟨"%42"⟩;dropfelt ⟨"%45"⟩;Code.part24;dropfelt ⟨"%13"⟩;dropfelt ⟨"%46"⟩;dropfelt ⟨"%47"⟩;dropfelt ⟨"%48"⟩;Code.part25;dropfelt ⟨"%43"⟩;dropfelt ⟨"%49"⟩;dropfelt ⟨"%44"⟩;dropfelt ⟨"%50"⟩;dropfelt ⟨"%51"⟩;Code.part26;dropfelt ⟨"%22"⟩;dropfelt ⟨"%52"⟩;dropfelt ⟨"%41"⟩;dropfelt ⟨"%53"⟩;dropfelt ⟨"%54"⟩;Code.part27;dropfelt ⟨"%7"⟩;dropfelt ⟨"%56"⟩;dropfelt ⟨"%59"⟩;Code.part28;dropfelt ⟨"%15"⟩;dropfelt ⟨"%60"⟩;dropfelt ⟨"%58"⟩;dropfelt ⟨"%61"⟩;dropfelt ⟨"%63"⟩;Code.part29;dropfelt ⟨"%57"⟩;dropfelt ⟨"%62"⟩;dropfelt ⟨"%64"⟩;dropfelt ⟨"%65"⟩;dropfelt ⟨"%66"⟩;dropfelt ⟨"%55"⟩;Code.part30;dropfelt ⟨"%19"⟩;dropfelt ⟨"%21"⟩;dropfelt ⟨"%67"⟩;dropfelt ⟨"%68"⟩;dropfelt ⟨"%70"⟩;Code.part31;dropfelt ⟨"%20"⟩;dropfelt ⟨"%71"⟩;dropfelt ⟨"%69"⟩;dropfelt ⟨"%72"⟩;dropfelt ⟨"%73"⟩) = prog
   unfold Code.part18
   MLIR
   rewrite [←eq]
-  unfold part18_state_update part18_state
+  rewrite [MLIR.run_seq_def,MLIR.run_dropfelt]
+  unfold part18_state_update part18_drops part18_state
   rfl
 
 lemma part18_updates_opaque {st : State} : 
   Code.getReturn (part17_state_update st) = [y0, y1, y2, y3, y4, y5, y6, y7, y8, y9, y10, y11, y12, y13, y14, y15, y16, y17] ↔
-  Code.getReturn (part18_state_update (part17_state st)) = [y0, y1, y2, y3, y4, y5, y6, y7, y8, y9, y10, y11, y12, y13, y14, y15, y16, y17] := by
+  Code.getReturn (part18_state_update (part17_drops (part17_state st))) = [y0, y1, y2, y3, y4, y5, y6, y7, y8, y9, y10, y11, y12, y13, y14, y15, y16, y17] := by
   simp [part17_state_update, part18_wp]
 
 end Risc0.ComputeDecode.Witness.WP
