Risc0/Gadgets/ComputeDecode/Witness/WeakestPresPart24.lean
@@ -10,42 +10,37 @@ open MLIRNotation
 -- The state obtained by running Code.part24 on st
 def part24_state (st: State) : State :=
   
-          ((((st["%45"] ←ₛ getImpl st { name := "data" } 0 2)[felts][{ name := "%46" }] ←
-                Option.get! (State.felts (st["%45"] ←ₛ getImpl st { name := "data" } 0 2) { name := "%45" }) *
-                  Option.get! (State.felts st { name := "%11" }))["%47"] ←ₛ
-              getImpl st { name := "data" } 0 12)[felts][{ name := "%48" }] ←
-            Option.get!
-                (State.felts
-                  (((st["%45"] ←ₛ getImpl st { name := "data" } 0 2)[felts][{ name := "%46" }] ←
-                      Option.get! (State.felts (st["%45"] ←ₛ getImpl st { name := "data" } 0 2) { name := "%45" }) *
-                        Option.get! (State.felts st { name := "%11" }))["%47"] ←ₛ
-                    getImpl st { name := "data" } 0 12)
-                  { name := "%47" }) *
-              Option.get!
-                (State.felts st
-                  {
-                    name :=
-                      "%13" })) 
+          ((((st["%47"] ←ₛ getImpl st { name := "data" } 0 12)[felts][{ name := "%48" }] ←
+                Option.get! (State.felts (st["%47"] ←ₛ getImpl st { name := "data" } 0 12) { name := "%47" }) *
+                  Option.get! (State.felts st { name := "%13" }))[felts][{ name := "%49" }] ←
+              Option.get! (State.felts (st["%47"] ←ₛ getImpl st { name := "data" } 0 12) { name := "%47" }) *
+                  Option.get! (State.felts st { name := "%13" }) +
+                Option.get! (State.felts st { name := "%46" }))["%44"] ←ₛ
+            getImpl st { name := "data" } 0 11) 
+
+def part24_drops (st: State) : State :=
+  State.dropFelts (State.dropFelts (State.dropFelts (State.dropFelts (st) ⟨"%13"⟩) ⟨"%46"⟩) ⟨"%47"⟩) ⟨"%48"⟩
 
 -- Run the program from part24 onwards by using part24_state rather than Code.part24
 def part24_state_update (st: State): State :=
-  Γ (part24_state st) ⟦Code.part25; Code.part26; Code.part27; Code.part28; Code.part29; Code.part30; Code.part31⟧
+  Γ (part24_drops (part24_state st)) ⟦Code.part25;dropfelt ⟨"%43"⟩;dropfelt ⟨"%49"⟩;dropfelt ⟨"%44"⟩;dropfelt ⟨"%50"⟩;dropfelt ⟨"%51"⟩;Code.part26;dropfelt ⟨"%22"⟩;dropfelt ⟨"%52"⟩;dropfelt ⟨"%41"⟩;dropfelt ⟨"%53"⟩;dropfelt ⟨"%54"⟩;Code.part27;dropfelt ⟨"%7"⟩;dropfelt ⟨"%56"⟩;dropfelt ⟨"%59"⟩;Code.part28;dropfelt ⟨"%15"⟩;dropfelt ⟨"%60"⟩;dropfelt ⟨"%58"⟩;dropfelt ⟨"%61"⟩;dropfelt ⟨"%63"⟩;Code.part29;dropfelt ⟨"%57"⟩;dropfelt ⟨"%62"⟩;dropfelt ⟨"%64"⟩;dropfelt ⟨"%65"⟩;dropfelt ⟨"%66"⟩;dropfelt ⟨"%55"⟩;Code.part30;dropfelt ⟨"%19"⟩;dropfelt ⟨"%21"⟩;dropfelt ⟨"%67"⟩;dropfelt ⟨"%68"⟩;dropfelt ⟨"%70"⟩;Code.part31;dropfelt ⟨"%20"⟩;dropfelt ⟨"%71"⟩;dropfelt ⟨"%69"⟩;dropfelt ⟨"%72"⟩;dropfelt ⟨"%73"⟩⟧
 
 -- Prove that substituting part24_state for Code.part24 produces the same result
 lemma part24_wp {st : State} {y0 y1 y2 y3 y4 y5 y6 y7 y8 y9 y10 y11 y12 y13 y14 y15 y16 y17 : Option Felt} :
-  Code.getReturn (MLIR.runProgram (Code.part24; Code.part25; Code.part26; Code.part27; Code.part28; Code.part29; Code.part30; Code.part31) st) = [y0, y1, y2, y3, y4, y5, y6, y7, y8, y9, y10, y11, y12, y13, y14, y15, y16, y17] ↔
+  Code.getReturn (MLIR.runProgram (Code.part24;dropfelt ⟨"%13"⟩;dropfelt ⟨"%46"⟩;dropfelt ⟨"%47"⟩;dropfelt ⟨"%48"⟩;Code.part25;dropfelt ⟨"%43"⟩;dropfelt ⟨"%49"⟩;dropfelt ⟨"%44"⟩;dropfelt ⟨"%50"⟩;dropfelt ⟨"%51"⟩;Code.part26;dropfelt ⟨"%22"⟩;dropfelt ⟨"%52"⟩;dropfelt ⟨"%41"⟩;dropfelt ⟨"%53"⟩;dropfelt ⟨"%54"⟩;Code.part27;dropfelt ⟨"%7"⟩;dropfelt ⟨"%56"⟩;dropfelt ⟨"%59"⟩;Code.part28;dropfelt ⟨"%15"⟩;dropfelt ⟨"%60"⟩;dropfelt ⟨"%58"⟩;dropfelt ⟨"%61"⟩;dropfelt ⟨"%63"⟩;Code.part29;dropfelt ⟨"%57"⟩;dropfelt ⟨"%62"⟩;dropfelt ⟨"%64"⟩;dropfelt ⟨"%65"⟩;dropfelt ⟨"%66"⟩;dropfelt ⟨"%55"⟩;Code.part30;dropfelt ⟨"%19"⟩;dropfelt ⟨"%21"⟩;dropfelt ⟨"%67"⟩;dropfelt ⟨"%68"⟩;dropfelt ⟨"%70"⟩;Code.part31;dropfelt ⟨"%20"⟩;dropfelt ⟨"%71"⟩;dropfelt ⟨"%69"⟩;dropfelt ⟨"%72"⟩;dropfelt ⟨"%73"⟩) st) = [y0, y1, y2, y3, y4, y5, y6, y7, y8, y9, y10, y11, y12, y13, y14, y15, y16, y17] ↔
   Code.getReturn (part24_state_update st) = [y0, y1, y2, y3, y4, y5, y6, y7, y8, y9, y10, y11, y12, y13, y14, y15, y16, y17] := by
   unfold MLIR.runProgram; simp only
-  generalize eq : (Code.part25; Code.part26; Code.part27; Code.part28; Code.part29; Code.part30; Code.part31) = prog
+  generalize eq : (dropfelt ⟨"%13"⟩;dropfelt ⟨"%46"⟩;dropfelt ⟨"%47"⟩;dropfelt ⟨"%48"⟩;Code.part25;dropfelt ⟨"%43"⟩;dropfelt ⟨"%49"⟩;dropfelt ⟨"%44"⟩;dropfelt ⟨"%50"⟩;dropfelt ⟨"%51"⟩;Code.part26;dropfelt ⟨"%22"⟩;dropfelt ⟨"%52"⟩;dropfelt ⟨"%41"⟩;dropfelt ⟨"%53"⟩;dropfelt ⟨"%54"⟩;Code.part27;dropfelt ⟨"%7"⟩;dropfelt ⟨"%56"⟩;dropfelt ⟨"%59"⟩;Code.part28;dropfelt ⟨"%15"⟩;dropfelt ⟨"%60"⟩;dropfelt ⟨"%58"⟩;dropfelt ⟨"%61"⟩;dropfelt ⟨"%63"⟩;Code.part29;dropfelt ⟨"%57"⟩;dropfelt ⟨"%62"⟩;dropfelt ⟨"%64"⟩;dropfelt ⟨"%65"⟩;dropfelt ⟨"%66"⟩;dropfelt ⟨"%55"⟩;Code.part30;dropfelt ⟨"%19"⟩;dropfelt ⟨"%21"⟩;dropfelt ⟨"%67"⟩;dropfelt ⟨"%68"⟩;dropfelt ⟨"%70"⟩;Code.part31;dropfelt ⟨"%20"⟩;dropfelt ⟨"%71"⟩;dropfelt ⟨"%69"⟩;dropfelt ⟨"%72"⟩;dropfelt ⟨"%73"⟩) = prog
   unfold Code.part24
   MLIR
   rewrite [←eq]
-  unfold part24_state_update part24_state
+  rewrite [MLIR.run_seq_def,MLIR.run_dropfelt, MLIR.run_seq_def,MLIR.run_dropfelt, MLIR.run_seq_def,MLIR.run_dropfelt, MLIR.run_seq_def,MLIR.run_dropfelt]
+  unfold part24_state_update part24_drops part24_state
   rfl
 
 lemma part24_updates_opaque {st : State} : 
   Code.getReturn (part23_state_update st) = [y0, y1, y2, y3, y4, y5, y6, y7, y8, y9, y10, y11, y12, y13, y14, y15, y16, y17] ↔
-  Code.getReturn (part24_state_update (part23_state st)) = [y0, y1, y2, y3, y4, y5, y6, y7, y8, y9, y10, y11, y12, y13, y14, y15, y16, y17] := by
+  Code.getReturn (part24_state_update (part23_drops (part23_state st))) = [y0, y1, y2, y3, y4, y5, y6, y7, y8, y9, y10, y11, y12, y13, y14, y15, y16, y17] := by
   simp [part23_state_update, part24_wp]
 
 end Risc0.ComputeDecode.Witness.WP
