Risc0/Gadgets/ComputeDecode/Witness/WeakestPresPart28.lean
@@ -10,35 +10,47 @@ open MLIRNotation
 -- The state obtained by running Code.part28 on st
 def part28_state (st: State) : State :=
   
-          ((((st[felts][{ name := "%60" }] ←
-                  Option.get! (State.felts st { name := "%59" }) *
-                    Option.get! (State.felts st { name := "%7" }))[felts][{ name := "%61" }] ←
-                Option.get! (State.felts st { name := "%59" }) * Option.get! (State.felts st { name := "%7" }) +
-                  Option.get! (State.felts st { name := "%58" }))[felts][{ name := "%62" }] ←
-              (Option.get! (State.felts st { name := "%59" }) * Option.get! (State.felts st { name := "%7" }) +
-                  Option.get! (State.felts st { name := "%58" })) *
-                Option.get! (State.felts st { name := "%15" }))["%63"] ←ₛ
-            getImpl st { name := "data" } 0 14) 
+          ((((st[felts][{ name := "%61" }] ←
+                  Option.get! (State.felts st { name := "%60" }) +
+                    Option.get! (State.felts st { name := "%58" }))[felts][{ name := "%62" }] ←
+                (Option.get! (State.felts st { name := "%60" }) + Option.get! (State.felts st { name := "%58" })) *
+                  Option.get! (State.felts st { name := "%15" }))["%63"] ←ₛ
+              getImpl st { name := "data" } 0 14)[felts][{ name := "%64" }] ←
+            Option.get!
+                (State.felts
+                  (((st[felts][{ name := "%61" }] ←
+                        Option.get! (State.felts st { name := "%60" }) +
+                          Option.get! (State.felts st { name := "%58" }))[felts][{ name := "%62" }] ←
+                      (Option.get! (State.felts st { name := "%60" }) +
+                          Option.get! (State.felts st { name := "%58" })) *
+                        Option.get! (State.felts st { name := "%15" }))["%63"] ←ₛ
+                    getImpl st { name := "data" } 0 14)
+                  { name := "%63" }) *
+              Option.get! (State.felts st { name := "%19" })) 
+
+def part28_drops (st: State) : State :=
+  State.dropFelts (State.dropFelts (State.dropFelts (State.dropFelts (State.dropFelts (st) ⟨"%15"⟩) ⟨"%60"⟩) ⟨"%58"⟩) ⟨"%61"⟩) ⟨"%63"⟩
 
 -- Run the program from part28 onwards by using part28_state rather than Code.part28
 def part28_state_update (st: State): State :=
-  Γ (part28_state st) ⟦Code.part29; Code.part30; Code.part31⟧
+  Γ (part28_drops (part28_state st)) ⟦Code.part29;dropfelt ⟨"%57"⟩;dropfelt ⟨"%62"⟩;dropfelt ⟨"%64"⟩;dropfelt ⟨"%65"⟩;dropfelt ⟨"%66"⟩;dropfelt ⟨"%55"⟩;Code.part30;dropfelt ⟨"%19"⟩;dropfelt ⟨"%21"⟩;dropfelt ⟨"%67"⟩;dropfelt ⟨"%68"⟩;dropfelt ⟨"%70"⟩;Code.part31;dropfelt ⟨"%20"⟩;dropfelt ⟨"%71"⟩;dropfelt ⟨"%69"⟩;dropfelt ⟨"%72"⟩;dropfelt ⟨"%73"⟩⟧
 
 -- Prove that substituting part28_state for Code.part28 produces the same result
 lemma part28_wp {st : State} {y0 y1 y2 y3 y4 y5 y6 y7 y8 y9 y10 y11 y12 y13 y14 y15 y16 y17 : Option Felt} :
-  Code.getReturn (MLIR.runProgram (Code.part28; Code.part29; Code.part30; Code.part31) st) = [y0, y1, y2, y3, y4, y5, y6, y7, y8, y9, y10, y11, y12, y13, y14, y15, y16, y17] ↔
+  Code.getReturn (MLIR.runProgram (Code.part28;dropfelt ⟨"%15"⟩;dropfelt ⟨"%60"⟩;dropfelt ⟨"%58"⟩;dropfelt ⟨"%61"⟩;dropfelt ⟨"%63"⟩;Code.part29;dropfelt ⟨"%57"⟩;dropfelt ⟨"%62"⟩;dropfelt ⟨"%64"⟩;dropfelt ⟨"%65"⟩;dropfelt ⟨"%66"⟩;dropfelt ⟨"%55"⟩;Code.part30;dropfelt ⟨"%19"⟩;dropfelt ⟨"%21"⟩;dropfelt ⟨"%67"⟩;dropfelt ⟨"%68"⟩;dropfelt ⟨"%70"⟩;Code.part31;dropfelt ⟨"%20"⟩;dropfelt ⟨"%71"⟩;dropfelt ⟨"%69"⟩;dropfelt ⟨"%72"⟩;dropfelt ⟨"%73"⟩) st) = [y0, y1, y2, y3, y4, y5, y6, y7, y8, y9, y10, y11, y12, y13, y14, y15, y16, y17] ↔
   Code.getReturn (part28_state_update st) = [y0, y1, y2, y3, y4, y5, y6, y7, y8, y9, y10, y11, y12, y13, y14, y15, y16, y17] := by
   unfold MLIR.runProgram; simp only
-  generalize eq : (Code.part29; Code.part30; Code.part31) = prog
+  generalize eq : (dropfelt ⟨"%15"⟩;dropfelt ⟨"%60"⟩;dropfelt ⟨"%58"⟩;dropfelt ⟨"%61"⟩;dropfelt ⟨"%63"⟩;Code.part29;dropfelt ⟨"%57"⟩;dropfelt ⟨"%62"⟩;dropfelt ⟨"%64"⟩;dropfelt ⟨"%65"⟩;dropfelt ⟨"%66"⟩;dropfelt ⟨"%55"⟩;Code.part30;dropfelt ⟨"%19"⟩;dropfelt ⟨"%21"⟩;dropfelt ⟨"%67"⟩;dropfelt ⟨"%68"⟩;dropfelt ⟨"%70"⟩;Code.part31;dropfelt ⟨"%20"⟩;dropfelt ⟨"%71"⟩;dropfelt ⟨"%69"⟩;dropfelt ⟨"%72"⟩;dropfelt ⟨"%73"⟩) = prog
   unfold Code.part28
   MLIR
   rewrite [←eq]
-  unfold part28_state_update part28_state
+  rewrite [MLIR.run_seq_def,MLIR.run_dropfelt, MLIR.run_seq_def,MLIR.run_dropfelt, MLIR.run_seq_def,MLIR.run_dropfelt, MLIR.run_seq_def,MLIR.run_dropfelt, MLIR.run_seq_def,MLIR.run_dropfelt]
+  unfold part28_state_update part28_drops part28_state
   rfl
 
 lemma part28_updates_opaque {st : State} : 
   Code.getReturn (part27_state_update st) = [y0, y1, y2, y3, y4, y5, y6, y7, y8, y9, y10, y11, y12, y13, y14, y15, y16, y17] ↔
-  Code.getReturn (part28_state_update (part27_state st)) = [y0, y1, y2, y3, y4, y5, y6, y7, y8, y9, y10, y11, y12, y13, y14, y15, y16, y17] := by
+  Code.getReturn (part28_state_update (part27_drops (part27_state st))) = [y0, y1, y2, y3, y4, y5, y6, y7, y8, y9, y10, y11, y12, y13, y14, y15, y16, y17] := by
   simp [part27_state_update, part28_wp]
 
 end Risc0.ComputeDecode.Witness.WP
