Risc0/Gadgets/ComputeDecode/Witness/WeakestPresPart29.lean
@@ -10,38 +10,47 @@ open MLIRNotation
 -- The state obtained by running Code.part29 on st
 def part29_state (st: State) : State :=
   
-          ((((st[felts][{ name := "%64" }] ←
-                  Option.get! (State.felts st { name := "%63" }) *
-                    Option.get! (State.felts st { name := "%19" }))[felts][{ name := "%65" }] ←
-                Option.get! (State.felts st { name := "%63" }) * Option.get! (State.felts st { name := "%19" }) +
-                  Option.get! (State.felts st { name := "%62" }))[felts][{ name := "%66" }] ←
-              Option.get! (State.felts st { name := "%63" }) * Option.get! (State.felts st { name := "%19" }) +
-                  Option.get! (State.felts st { name := "%62" }) +
-                Option.get! (State.felts st { name := "%57" }))[felts][{ name := "%67" }] ←
-            Option.get! (State.felts st { name := "%63" }) * Option.get! (State.felts st { name := "%19" }) +
-                  Option.get! (State.felts st { name := "%62" }) +
+          ((((st[felts][{ name := "%65" }] ←
+                  Option.get! (State.felts st { name := "%64" }) +
+                    Option.get! (State.felts st { name := "%62" }))[felts][{ name := "%66" }] ←
+                Option.get! (State.felts st { name := "%64" }) + Option.get! (State.felts st { name := "%62" }) +
+                  Option.get! (State.felts st { name := "%57" }))["%55"] ←ₛ
+              getImpl st { name := "data" } 0 6)[felts][{ name := "%67" }] ←
+            Option.get! (State.felts st { name := "%64" }) + Option.get! (State.felts st { name := "%62" }) +
                 Option.get! (State.felts st { name := "%57" }) +
-              Option.get! (State.felts st { name := "%55" })) 
+              Option.get!
+                (State.felts
+                  (((st[felts][{ name := "%65" }] ←
+                        Option.get! (State.felts st { name := "%64" }) +
+                          Option.get! (State.felts st { name := "%62" }))[felts][{ name := "%66" }] ←
+                      Option.get! (State.felts st { name := "%64" }) + Option.get! (State.felts st { name := "%62" }) +
+                        Option.get! (State.felts st { name := "%57" }))["%55"] ←ₛ
+                    getImpl st { name := "data" } 0 6)
+                  { name := "%55" })) 
+
+def part29_drops (st: State) : State :=
+  State.dropFelts (State.dropFelts (State.dropFelts (State.dropFelts (State.dropFelts (State.dropFelts (st) ⟨"%57"⟩) ⟨"%62"⟩) ⟨"%64"⟩) ⟨"%65"⟩) ⟨"%66"⟩) ⟨"%55"⟩
 
 -- Run the program from part29 onwards by using part29_state rather than Code.part29
 def part29_state_update (st: State): State :=
-  Γ (part29_state st) ⟦Code.part30; Code.part31⟧
+  Γ (part29_drops (part29_state st)) ⟦Code.part30;dropfelt ⟨"%19"⟩;dropfelt ⟨"%21"⟩;dropfelt ⟨"%67"⟩;dropfelt ⟨"%68"⟩;dropfelt ⟨"%70"⟩;Code.part31;dropfelt ⟨"%20"⟩;dropfelt ⟨"%71"⟩;dropfelt ⟨"%69"⟩;dropfelt ⟨"%72"⟩;dropfelt ⟨"%73"⟩⟧
 
 -- Prove that substituting part29_state for Code.part29 produces the same result
 lemma part29_wp {st : State} {y0 y1 y2 y3 y4 y5 y6 y7 y8 y9 y10 y11 y12 y13 y14 y15 y16 y17 : Option Felt} :
-  Code.getReturn (MLIR.runProgram (Code.part29; Code.part30; Code.part31) st) = [y0, y1, y2, y3, y4, y5, y6, y7, y8, y9, y10, y11, y12, y13, y14, y15, y16, y17] ↔
+  Code.getReturn (MLIR.runProgram (Code.part29;dropfelt ⟨"%57"⟩;dropfelt ⟨"%62"⟩;dropfelt ⟨"%64"⟩;dropfelt ⟨"%65"⟩;dropfelt ⟨"%66"⟩;dropfelt ⟨"%55"⟩;Code.part30;dropfelt ⟨"%19"⟩;dropfelt ⟨"%21"⟩;dropfelt ⟨"%67"⟩;dropfelt ⟨"%68"⟩;dropfelt ⟨"%70"⟩;Code.part31;dropfelt ⟨"%20"⟩;dropfelt ⟨"%71"⟩;dropfelt ⟨"%69"⟩;dropfelt ⟨"%72"⟩;dropfelt ⟨"%73"⟩) st) = [y0, y1, y2, y3, y4, y5, y6, y7, y8, y9, y10, y11, y12, y13, y14, y15, y16, y17] ↔
   Code.getReturn (part29_state_update st) = [y0, y1, y2, y3, y4, y5, y6, y7, y8, y9, y10, y11, y12, y13, y14, y15, y16, y17] := by
   unfold MLIR.runProgram; simp only
-  generalize eq : (Code.part30; Code.part31) = prog
+  generalize eq : (dropfelt ⟨"%57"⟩;dropfelt ⟨"%62"⟩;dropfelt ⟨"%64"⟩;dropfelt ⟨"%65"⟩;dropfelt ⟨"%66"⟩;dropfelt ⟨"%55"⟩;Code.part30;dropfelt ⟨"%19"⟩;dropfelt ⟨"%21"⟩;dropfelt ⟨"%67"⟩;dropfelt ⟨"%68"⟩;dropfelt ⟨"%70"⟩;Code.part31;dropfelt ⟨"%20"⟩;dropfelt ⟨"%71"⟩;dropfelt ⟨"%69"⟩;dropfelt ⟨"%72"⟩;dropfelt ⟨"%73"⟩) = prog
   unfold Code.part29
   MLIR
   rewrite [←eq]
-  unfold part29_state_update part29_state
+  rewrite [MLIR.run_seq_def,MLIR.run_dropfelt, MLIR.run_seq_def,MLIR.run_dropfelt, MLIR.run_seq_def,MLIR.run_dropfelt, MLIR.run_seq_def,MLIR.run_dropfelt, MLIR.run_seq_def,MLIR.run_dropfelt, MLIR.run_seq_def,MLIR.run_dropfelt]
+  unfold part29_state_update part29_drops part29_state
   rfl
 
 lemma part29_updates_opaque {st : State} : 
   Code.getReturn (part28_state_update st) = [y0, y1, y2, y3, y4, y5, y6, y7, y8, y9, y10, y11, y12, y13, y14, y15, y16, y17] ↔
-  Code.getReturn (part29_state_update (part28_state st)) = [y0, y1, y2, y3, y4, y5, y6, y7, y8, y9, y10, y11, y12, y13, y14, y15, y16, y17] := by
+  Code.getReturn (part29_state_update (part28_drops (part28_state st))) = [y0, y1, y2, y3, y4, y5, y6, y7, y8, y9, y10, y11, y12, y13, y14, y15, y16, y17] := by
   simp [part28_state_update, part29_wp]
 
 end Risc0.ComputeDecode.Witness.WP
