Risc0/Gadgets/ComputeDecode/Witness/WeakestPresPart30.lean
@@ -14,34 +14,42 @@ def part30_state (st: State) : State :=
                 (Option.get! (State.felts st { name := "%21" }) - Option.get! (State.felts st { name := "%67" }))
                 (st[felts][{ name := "%68" }] ←
                   Option.get! (State.felts st { name := "%21" }) -
-                    Option.get! (State.felts st { name := "%67" })))["%69"] ←ₛ
-              getImpl st { name := "data" } 0 17)["%70"] ←ₛ
-            getImpl
-              (withEqZero
-                (Option.get! (State.felts st { name := "%21" }) - Option.get! (State.felts st { name := "%67" }))
-                (st[felts][{ name := "%68" }] ←
-                  Option.get! (State.felts st { name := "%21" }) - Option.get! (State.felts st { name := "%67" })))
-              { name := "data" } 0 16) 
+                    Option.get! (State.felts st { name := "%67" })))["%70"] ←ₛ
+              getImpl st { name := "data" } 0 16)[felts][{ name := "%71" }] ←
+            Option.get!
+                (State.felts
+                  ((withEqZero
+                      (Option.get! (State.felts st { name := "%21" }) - Option.get! (State.felts st { name := "%67" }))
+                      (st[felts][{ name := "%68" }] ←
+                        Option.get! (State.felts st { name := "%21" }) -
+                          Option.get! (State.felts st { name := "%67" })))["%70"] ←ₛ
+                    getImpl st { name := "data" } 0 16)
+                  { name := "%70" }) *
+              Option.get! (State.felts st { name := "%19" })) 
+
+def part30_drops (st: State) : State :=
+  State.dropFelts (State.dropFelts (State.dropFelts (State.dropFelts (State.dropFelts (st) ⟨"%19"⟩) ⟨"%21"⟩) ⟨"%67"⟩) ⟨"%68"⟩) ⟨"%70"⟩
 
 -- Run the program from part30 onwards by using part30_state rather than Code.part30
 def part30_state_update (st: State): State :=
-  Γ (part30_state st) ⟦Code.part31⟧
+  Γ (part30_drops (part30_state st)) ⟦Code.part31;dropfelt ⟨"%20"⟩;dropfelt ⟨"%71"⟩;dropfelt ⟨"%69"⟩;dropfelt ⟨"%72"⟩;dropfelt ⟨"%73"⟩⟧
 
 -- Prove that substituting part30_state for Code.part30 produces the same result
 lemma part30_wp {st : State} {y0 y1 y2 y3 y4 y5 y6 y7 y8 y9 y10 y11 y12 y13 y14 y15 y16 y17 : Option Felt} :
-  Code.getReturn (MLIR.runProgram (Code.part30; Code.part31) st) = [y0, y1, y2, y3, y4, y5, y6, y7, y8, y9, y10, y11, y12, y13, y14, y15, y16, y17] ↔
+  Code.getReturn (MLIR.runProgram (Code.part30;dropfelt ⟨"%19"⟩;dropfelt ⟨"%21"⟩;dropfelt ⟨"%67"⟩;dropfelt ⟨"%68"⟩;dropfelt ⟨"%70"⟩;Code.part31;dropfelt ⟨"%20"⟩;dropfelt ⟨"%71"⟩;dropfelt ⟨"%69"⟩;dropfelt ⟨"%72"⟩;dropfelt ⟨"%73"⟩) st) = [y0, y1, y2, y3, y4, y5, y6, y7, y8, y9, y10, y11, y12, y13, y14, y15, y16, y17] ↔
   Code.getReturn (part30_state_update st) = [y0, y1, y2, y3, y4, y5, y6, y7, y8, y9, y10, y11, y12, y13, y14, y15, y16, y17] := by
   unfold MLIR.runProgram; simp only
-  generalize eq : (Code.part31) = prog
+  generalize eq : (dropfelt ⟨"%19"⟩;dropfelt ⟨"%21"⟩;dropfelt ⟨"%67"⟩;dropfelt ⟨"%68"⟩;dropfelt ⟨"%70"⟩;Code.part31;dropfelt ⟨"%20"⟩;dropfelt ⟨"%71"⟩;dropfelt ⟨"%69"⟩;dropfelt ⟨"%72"⟩;dropfelt ⟨"%73"⟩) = prog
   unfold Code.part30
   MLIR
   rewrite [←eq]
-  unfold part30_state_update part30_state
+  rewrite [MLIR.run_seq_def,MLIR.run_dropfelt, MLIR.run_seq_def,MLIR.run_dropfelt, MLIR.run_seq_def,MLIR.run_dropfelt, MLIR.run_seq_def,MLIR.run_dropfelt, MLIR.run_seq_def,MLIR.run_dropfelt]
+  unfold part30_state_update part30_drops part30_state
   rfl
 
 lemma part30_updates_opaque {st : State} : 
   Code.getReturn (part29_state_update st) = [y0, y1, y2, y3, y4, y5, y6, y7, y8, y9, y10, y11, y12, y13, y14, y15, y16, y17] ↔
-  Code.getReturn (part30_state_update (part29_state st)) = [y0, y1, y2, y3, y4, y5, y6, y7, y8, y9, y10, y11, y12, y13, y14, y15, y16, y17] := by
+  Code.getReturn (part30_state_update (part29_drops (part29_state st))) = [y0, y1, y2, y3, y4, y5, y6, y7, y8, y9, y10, y11, y12, y13, y14, y15, y16, y17] := by
   simp [part29_state_update, part30_wp]
 
 end Risc0.ComputeDecode.Witness.WP
