Risc0/Gadgets/ComputeDecode/Witness/WeakestPresPart31.lean
@@ -8,34 +8,45 @@ namespace Risc0.ComputeDecode.Witness.WP
 open MLIRNotation
 
 -- The state obtained by running Code.part31 on st
-def part31_state (st: State) : State := 
+def part31_state (st: State) : State :=
   
-        (withEqZero
-          (Option.get! (State.felts st { name := "%20" }) -
-            (Option.get! (State.felts st { name := "%70" }) * Option.get! (State.felts st { name := "%19" }) +
-              Option.get! (State.felts st { name := "%69" })))
-          (((st[felts][{ name := "%71" }] ←
-                Option.get! (State.felts st { name := "%70" }) *
-                  Option.get! (State.felts st { name := "%19" }))[felts][{ name := "%72" }] ←
-              Option.get! (State.felts st { name := "%70" }) * Option.get! (State.felts st { name := "%19" }) +
-                Option.get! (State.felts st { name := "%69" }))[felts][{ name := "%73" }] ←
-            Option.get! (State.felts st { name := "%20" }) -
-              (Option.get! (State.felts st { name := "%70" }) * Option.get! (State.felts st { name := "%19" }) +
-                Option.get! (State.felts st { name := "%69" })))) 
+          (withEqZero
+            (Option.get! (State.felts st { name := "%20" }) -
+              (Option.get! (State.felts st { name := "%71" }) +
+                Option.get! (State.felts (st["%69"] ←ₛ getImpl st { name := "data" } 0 17) { name := "%69" })))
+            (((st["%69"] ←ₛ getImpl st { name := "data" } 0 17)[felts][{ name := "%72" }] ←
+                Option.get! (State.felts st { name := "%71" }) +
+                  Option.get!
+                    (State.felts (st["%69"] ←ₛ getImpl st { name := "data" } 0 17)
+                      { name := "%69" }))[felts][{ name := "%73" }] ←
+              Option.get! (State.felts st { name := "%20" }) -
+                (Option.get! (State.felts st { name := "%71" }) +
+                  Option.get!
+                    (State.felts (st["%69"] ←ₛ getImpl st { name := "data" } 0 17) { name := "%69" })))) 
+
+def part31_drops (st: State) : State :=
+  State.dropFelts (State.dropFelts (State.dropFelts (State.dropFelts (State.dropFelts (st) ⟨"%20"⟩) ⟨"%71"⟩) ⟨"%69"⟩) ⟨"%72"⟩) ⟨"%73"⟩
+
+-- Run the program from part31 onwards by using part31_state rather than Code.part31
+def part31_state_update (st: State): State :=
+  part31_drops (part31_state st)
 
 -- Prove that substituting part31_state for Code.part31 produces the same result
 lemma part31_wp {st : State} {y0 y1 y2 y3 y4 y5 y6 y7 y8 y9 y10 y11 y12 y13 y14 y15 y16 y17 : Option Felt} :
-  Code.getReturn (MLIR.runProgram Code.part31 st) = [y0, y1, y2, y3, y4, y5, y6, y7, y8, y9, y10, y11, y12, y13, y14, y15, y16, y17] ↔
-  Code.getReturn (part31_state st) = [y0, y1, y2, y3, y4, y5, y6, y7, y8, y9, y10, y11, y12, y13, y14, y15, y16, y17] := by
+  Code.getReturn (MLIR.runProgram (Code.part31;dropfelt ⟨"%20"⟩;dropfelt ⟨"%71"⟩;dropfelt ⟨"%69"⟩;dropfelt ⟨"%72"⟩;dropfelt ⟨"%73"⟩) st) = [y0, y1, y2, y3, y4, y5, y6, y7, y8, y9, y10, y11, y12, y13, y14, y15, y16, y17] ↔
+  Code.getReturn (part31_state_update st) = [y0, y1, y2, y3, y4, y5, y6, y7, y8, y9, y10, y11, y12, y13, y14, y15, y16, y17] := by
   unfold MLIR.runProgram; simp only
+  generalize eq : (dropfelt ⟨"%20"⟩;dropfelt ⟨"%71"⟩;dropfelt ⟨"%69"⟩;dropfelt ⟨"%72"⟩;dropfelt ⟨"%73"⟩) = prog
   unfold Code.part31
   MLIR
-  unfold part31_state
+  rewrite [←eq]
+  rewrite [MLIR.run_seq_def,MLIR.run_dropfelt, MLIR.run_seq_def,MLIR.run_dropfelt, MLIR.run_seq_def,MLIR.run_dropfelt, MLIR.run_seq_def,MLIR.run_dropfelt, MLIR.run_dropfelt]
+  unfold part31_state_update part31_drops part31_state
   rfl
 
 lemma part31_updates_opaque {st : State} : 
   Code.getReturn (part30_state_update st) = [y0, y1, y2, y3, y4, y5, y6, y7, y8, y9, y10, y11, y12, y13, y14, y15, y16, y17] ↔
-  Code.getReturn (part31_state (part30_state st)) = [y0, y1, y2, y3, y4, y5, y6, y7, y8, y9, y10, y11, y12, y13, y14, y15, y16, y17] := by
+  Code.getReturn (part31_state_update (part30_drops (part30_state st))) = [y0, y1, y2, y3, y4, y5, y6, y7, y8, y9, y10, y11, y12, y13, y14, y15, y16, y17] := by
   simp [part30_state_update, part31_wp]
 
 end Risc0.ComputeDecode.Witness.WP
