Risc0/Gadgets/ComputeDecode/Witness/WeakestPresPart7.lean
@@ -9,36 +9,51 @@ open MLIRNotation
 
 -- The state obtained by running Code.part7 on st
 def part7_state (st: State) : State :=
-  (State.set!
-              (st[felts][{ name := "%77" }] ←
-                Option.get! (State.felts st { name := "%76" }) * Option.get! (State.felts st { name := "%16" }))
-              { name := "data" } 1
-              (Option.get! (State.felts st { name := "%76" }) *
-                Option.get! (State.felts st { name := "%16" }))[felts][{ name := "%78" }] ←
-            feltBitAnd (Option.get! (State.felts st { name := "%23" }))
-              (Option.get! (State.felts st { name := "%15" })))[felts][{ name := "%79" }] ←
-          feltBitAnd (Option.get! (State.felts st { name := "%23" })) (Option.get! (State.felts st { name := "%15" })) *
-            Option.get! (State.felts st { name := "%14" })
+  
+          ((((State.set! st { name := "data" } 13 (Option.get! st.felts[({ name := "%84" }: FeltVar)]!))["%22"] ←ₛ
+                getImpl (State.set! st { name := "data" } 13 (Option.get! st.felts[({ name := "%84" }: FeltVar)]!))
+                  { name := "in" } 0 2)[felts][{ name := "%85" }] ←
+              feltBitAnd
+                (Option.get!
+                  (State.felts
+                    ((State.set! st { name := "data" } 13 (Option.get! st.felts[({ name := "%84" }: FeltVar)]!))["%22"] ←ₛ
+                      getImpl (State.set! st { name := "data" } 13 (Option.get! st.felts[({ name := "%84" }: FeltVar)]!))
+                        { name := "in" } 0 2)
+                    { name := "%22" }))
+                (Option.get! (State.felts st { name := "%19" })))[felts][{ name := "%86" }] ←
+            feltBitAnd
+                (Option.get!
+                  (State.felts
+                    ((State.set! st { name := "data" } 13 (Option.get! st.felts[({ name := "%84" }: FeltVar)]!))["%22"] ←ₛ
+                      getImpl (State.set! st { name := "data" } 13 (Option.get! st.felts[({ name := "%84" }: FeltVar)]!))
+                        { name := "in" } 0 2)
+                    { name := "%22" }))
+                (Option.get! (State.felts st { name := "%19" })) *
+              Option.get! (State.felts st { name := "%18" })) 
+
+def part7_drops (st: State) : State :=
+  State.dropFelts (State.dropFelts (st) ⟨"%84"⟩) ⟨"%85"⟩
 
 -- Run the program from part7 onwards by using part7_state rather than Code.part7
 def part7_state_update (st: State): State :=
-  Γ (part7_state st) ⟦Code.part8; Code.part9; Code.part10; Code.part11; Code.part12; Code.part13; Code.part14; Code.part15; Code.part16; Code.part17; Code.part18; Code.part19; Code.part20; Code.part21; Code.part22; Code.part23; Code.part24; Code.part25; Code.part26; Code.part27; Code.part28; Code.part29; Code.part30; Code.part31⟧
+  Γ (part7_drops (part7_state st)) ⟦Code.part8;dropfelt ⟨"%17"⟩;dropfelt ⟨"%16"⟩;dropfelt ⟨"%86"⟩;dropfelt ⟨"%87"⟩;dropfelt ⟨"%88"⟩;Code.part9;dropfelt ⟨"%89"⟩;dropfelt ⟨"%90"⟩;Code.part10;dropfelt ⟨"%91"⟩;dropfelt ⟨"%92"⟩;Code.part11;dropfelt ⟨"%93"⟩;Code.part12;dropfelt ⟨"%94"⟩;dropfelt ⟨"%95"⟩;Code.part13;dropfelt ⟨"%96"⟩;dropfelt ⟨"%2"⟩;dropfelt ⟨"%97"⟩;Code.part14;dropfelt ⟨"%14"⟩;dropfelt ⟨"%1"⟩;dropfelt ⟨"%98"⟩;dropfelt ⟨"%99"⟩;Code.part15;dropfelt ⟨"%6"⟩;dropfelt ⟨"%5"⟩;dropfelt ⟨"%4"⟩;dropfelt ⟨"%100"⟩;dropfelt ⟨"%101"⟩;Code.part16;dropfelt ⟨"%18"⟩;dropfelt ⟨"%102"⟩;dropfelt ⟨"%103"⟩;Code.part17;dropfelt ⟨"%104"⟩;dropfelt ⟨"%0"⟩;dropfelt ⟨"%105"⟩;Code.part18;dropfelt ⟨"%26"⟩;Code.part19;dropfelt ⟨"%28"⟩;dropfelt ⟨"%29"⟩;dropfelt ⟨"%30"⟩;dropfelt ⟨"%31"⟩;Code.part20;dropfelt ⟨"%27"⟩;dropfelt ⟨"%32"⟩;dropfelt ⟨"%33"⟩;dropfelt ⟨"%25"⟩;Code.part21;dropfelt ⟨"%3"⟩;dropfelt ⟨"%34"⟩;dropfelt ⟨"%35"⟩;dropfelt ⟨"%36"⟩;dropfelt ⟨"%37"⟩;Code.part22;dropfelt ⟨"%23"⟩;dropfelt ⟨"%38"⟩;dropfelt ⟨"%24"⟩;dropfelt ⟨"%39"⟩;dropfelt ⟨"%40"⟩;Code.part23;dropfelt ⟨"%11"⟩;dropfelt ⟨"%42"⟩;dropfelt ⟨"%45"⟩;Code.part24;dropfelt ⟨"%13"⟩;dropfelt ⟨"%46"⟩;dropfelt ⟨"%47"⟩;dropfelt ⟨"%48"⟩;Code.part25;dropfelt ⟨"%43"⟩;dropfelt ⟨"%49"⟩;dropfelt ⟨"%44"⟩;dropfelt ⟨"%50"⟩;dropfelt ⟨"%51"⟩;Code.part26;dropfelt ⟨"%22"⟩;dropfelt ⟨"%52"⟩;dropfelt ⟨"%41"⟩;dropfelt ⟨"%53"⟩;dropfelt ⟨"%54"⟩;Code.part27;dropfelt ⟨"%7"⟩;dropfelt ⟨"%56"⟩;dropfelt ⟨"%59"⟩;Code.part28;dropfelt ⟨"%15"⟩;dropfelt ⟨"%60"⟩;dropfelt ⟨"%58"⟩;dropfelt ⟨"%61"⟩;dropfelt ⟨"%63"⟩;Code.part29;dropfelt ⟨"%57"⟩;dropfelt ⟨"%62"⟩;dropfelt ⟨"%64"⟩;dropfelt ⟨"%65"⟩;dropfelt ⟨"%66"⟩;dropfelt ⟨"%55"⟩;Code.part30;dropfelt ⟨"%19"⟩;dropfelt ⟨"%21"⟩;dropfelt ⟨"%67"⟩;dropfelt ⟨"%68"⟩;dropfelt ⟨"%70"⟩;Code.part31;dropfelt ⟨"%20"⟩;dropfelt ⟨"%71"⟩;dropfelt ⟨"%69"⟩;dropfelt ⟨"%72"⟩;dropfelt ⟨"%73"⟩⟧
 
 -- Prove that substituting part7_state for Code.part7 produces the same result
 lemma part7_wp {st : State} {y0 y1 y2 y3 y4 y5 y6 y7 y8 y9 y10 y11 y12 y13 y14 y15 y16 y17 : Option Felt} :
-  Code.getReturn (MLIR.runProgram (Code.part7; Code.part8; Code.part9; Code.part10; Code.part11; Code.part12; Code.part13; Code.part14; Code.part15; Code.part16; Code.part17; Code.part18; Code.part19; Code.part20; Code.part21; Code.part22; Code.part23; Code.part24; Code.part25; Code.part26; Code.part27; Code.part28; Code.part29; Code.part30; Code.part31) st) = [y0, y1, y2, y3, y4, y5, y6, y7, y8, y9, y10, y11, y12, y13, y14, y15, y16, y17] ↔
+  Code.getReturn (MLIR.runProgram (Code.part7;dropfelt ⟨"%84"⟩;dropfelt ⟨"%85"⟩;Code.part8;dropfelt ⟨"%17"⟩;dropfelt ⟨"%16"⟩;dropfelt ⟨"%86"⟩;dropfelt ⟨"%87"⟩;dropfelt ⟨"%88"⟩;Code.part9;dropfelt ⟨"%89"⟩;dropfelt ⟨"%90"⟩;Code.part10;dropfelt ⟨"%91"⟩;dropfelt ⟨"%92"⟩;Code.part11;dropfelt ⟨"%93"⟩;Code.part12;dropfelt ⟨"%94"⟩;dropfelt ⟨"%95"⟩;Code.part13;dropfelt ⟨"%96"⟩;dropfelt ⟨"%2"⟩;dropfelt ⟨"%97"⟩;Code.part14;dropfelt ⟨"%14"⟩;dropfelt ⟨"%1"⟩;dropfelt ⟨"%98"⟩;dropfelt ⟨"%99"⟩;Code.part15;dropfelt ⟨"%6"⟩;dropfelt ⟨"%5"⟩;dropfelt ⟨"%4"⟩;dropfelt ⟨"%100"⟩;dropfelt ⟨"%101"⟩;Code.part16;dropfelt ⟨"%18"⟩;dropfelt ⟨"%102"⟩;dropfelt ⟨"%103"⟩;Code.part17;dropfelt ⟨"%104"⟩;dropfelt ⟨"%0"⟩;dropfelt ⟨"%105"⟩;Code.part18;dropfelt ⟨"%26"⟩;Code.part19;dropfelt ⟨"%28"⟩;dropfelt ⟨"%29"⟩;dropfelt ⟨"%30"⟩;dropfelt ⟨"%31"⟩;Code.part20;dropfelt ⟨"%27"⟩;dropfelt ⟨"%32"⟩;dropfelt ⟨"%33"⟩;dropfelt ⟨"%25"⟩;Code.part21;dropfelt ⟨"%3"⟩;dropfelt ⟨"%34"⟩;dropfelt ⟨"%35"⟩;dropfelt ⟨"%36"⟩;dropfelt ⟨"%37"⟩;Code.part22;dropfelt ⟨"%23"⟩;dropfelt ⟨"%38"⟩;dropfelt ⟨"%24"⟩;dropfelt ⟨"%39"⟩;dropfelt ⟨"%40"⟩;Code.part23;dropfelt ⟨"%11"⟩;dropfelt ⟨"%42"⟩;dropfelt ⟨"%45"⟩;Code.part24;dropfelt ⟨"%13"⟩;dropfelt ⟨"%46"⟩;dropfelt ⟨"%47"⟩;dropfelt ⟨"%48"⟩;Code.part25;dropfelt ⟨"%43"⟩;dropfelt ⟨"%49"⟩;dropfelt ⟨"%44"⟩;dropfelt ⟨"%50"⟩;dropfelt ⟨"%51"⟩;Code.part26;dropfelt ⟨"%22"⟩;dropfelt ⟨"%52"⟩;dropfelt ⟨"%41"⟩;dropfelt ⟨"%53"⟩;dropfelt ⟨"%54"⟩;Code.part27;dropfelt ⟨"%7"⟩;dropfelt ⟨"%56"⟩;dropfelt ⟨"%59"⟩;Code.part28;dropfelt ⟨"%15"⟩;dropfelt ⟨"%60"⟩;dropfelt ⟨"%58"⟩;dropfelt ⟨"%61"⟩;dropfelt ⟨"%63"⟩;Code.part29;dropfelt ⟨"%57"⟩;dropfelt ⟨"%62"⟩;dropfelt ⟨"%64"⟩;dropfelt ⟨"%65"⟩;dropfelt ⟨"%66"⟩;dropfelt ⟨"%55"⟩;Code.part30;dropfelt ⟨"%19"⟩;dropfelt ⟨"%21"⟩;dropfelt ⟨"%67"⟩;dropfelt ⟨"%68"⟩;dropfelt ⟨"%70"⟩;Code.part31;dropfelt ⟨"%20"⟩;dropfelt ⟨"%71"⟩;dropfelt ⟨"%69"⟩;dropfelt ⟨"%72"⟩;dropfelt ⟨"%73"⟩) st) = [y0, y1, y2, y3, y4, y5, y6, y7, y8, y9, y10, y11, y12, y13, y14, y15, y16, y17] ↔
   Code.getReturn (part7_state_update st) = [y0, y1, y2, y3, y4, y5, y6, y7, y8, y9, y10, y11, y12, y13, y14, y15, y16, y17] := by
   unfold MLIR.runProgram; simp only
-  generalize eq : (Code.part8; Code.part9; Code.part10; Code.part11; Code.part12; Code.part13; Code.part14; Code.part15; Code.part16; Code.part17; Code.part18; Code.part19; Code.part20; Code.part21; Code.part22; Code.part23; Code.part24; Code.part25; Code.part26; Code.part27; Code.part28; Code.part29; Code.part30; Code.part31) = prog
+  generalize eq : (dropfelt ⟨"%84"⟩;dropfelt ⟨"%85"⟩;Code.part8;dropfelt ⟨"%17"⟩;dropfelt ⟨"%16"⟩;dropfelt ⟨"%86"⟩;dropfelt ⟨"%87"⟩;dropfelt ⟨"%88"⟩;Code.part9;dropfelt ⟨"%89"⟩;dropfelt ⟨"%90"⟩;Code.part10;dropfelt ⟨"%91"⟩;dropfelt ⟨"%92"⟩;Code.part11;dropfelt ⟨"%93"⟩;Code.part12;dropfelt ⟨"%94"⟩;dropfelt ⟨"%95"⟩;Code.part13;dropfelt ⟨"%96"⟩;dropfelt ⟨"%2"⟩;dropfelt ⟨"%97"⟩;Code.part14;dropfelt ⟨"%14"⟩;dropfelt ⟨"%1"⟩;dropfelt ⟨"%98"⟩;dropfelt ⟨"%99"⟩;Code.part15;dropfelt ⟨"%6"⟩;dropfelt ⟨"%5"⟩;dropfelt ⟨"%4"⟩;dropfelt ⟨"%100"⟩;dropfelt ⟨"%101"⟩;Code.part16;dropfelt ⟨"%18"⟩;dropfelt ⟨"%102"⟩;dropfelt ⟨"%103"⟩;Code.part17;dropfelt ⟨"%104"⟩;dropfelt ⟨"%0"⟩;dropfelt ⟨"%105"⟩;Code.part18;dropfelt ⟨"%26"⟩;Code.part19;dropfelt ⟨"%28"⟩;dropfelt ⟨"%29"⟩;dropfelt ⟨"%30"⟩;dropfelt ⟨"%31"⟩;Code.part20;dropfelt ⟨"%27"⟩;dropfelt ⟨"%32"⟩;dropfelt ⟨"%33"⟩;dropfelt ⟨"%25"⟩;Code.part21;dropfelt ⟨"%3"⟩;dropfelt ⟨"%34"⟩;dropfelt ⟨"%35"⟩;dropfelt ⟨"%36"⟩;dropfelt ⟨"%37"⟩;Code.part22;dropfelt ⟨"%23"⟩;dropfelt ⟨"%38"⟩;dropfelt ⟨"%24"⟩;dropfelt ⟨"%39"⟩;dropfelt ⟨"%40"⟩;Code.part23;dropfelt ⟨"%11"⟩;dropfelt ⟨"%42"⟩;dropfelt ⟨"%45"⟩;Code.part24;dropfelt ⟨"%13"⟩;dropfelt ⟨"%46"⟩;dropfelt ⟨"%47"⟩;dropfelt ⟨"%48"⟩;Code.part25;dropfelt ⟨"%43"⟩;dropfelt ⟨"%49"⟩;dropfelt ⟨"%44"⟩;dropfelt ⟨"%50"⟩;dropfelt ⟨"%51"⟩;Code.part26;dropfelt ⟨"%22"⟩;dropfelt ⟨"%52"⟩;dropfelt ⟨"%41"⟩;dropfelt ⟨"%53"⟩;dropfelt ⟨"%54"⟩;Code.part27;dropfelt ⟨"%7"⟩;dropfelt ⟨"%56"⟩;dropfelt ⟨"%59"⟩;Code.part28;dropfelt ⟨"%15"⟩;dropfelt ⟨"%60"⟩;dropfelt ⟨"%58"⟩;dropfelt ⟨"%61"⟩;dropfelt ⟨"%63"⟩;Code.part29;dropfelt ⟨"%57"⟩;dropfelt ⟨"%62"⟩;dropfelt ⟨"%64"⟩;dropfelt ⟨"%65"⟩;dropfelt ⟨"%66"⟩;dropfelt ⟨"%55"⟩;Code.part30;dropfelt ⟨"%19"⟩;dropfelt ⟨"%21"⟩;dropfelt ⟨"%67"⟩;dropfelt ⟨"%68"⟩;dropfelt ⟨"%70"⟩;Code.part31;dropfelt ⟨"%20"⟩;dropfelt ⟨"%71"⟩;dropfelt ⟨"%69"⟩;dropfelt ⟨"%72"⟩;dropfelt ⟨"%73"⟩) = prog
   unfold Code.part7
   MLIR
   rewrite [←eq]
-  unfold part7_state_update part7_state
+  rewrite [MLIR.run_seq_def,MLIR.run_dropfelt, MLIR.run_seq_def,MLIR.run_dropfelt]
+  unfold part7_state_update part7_drops part7_state
   rfl
 
 lemma part7_updates_opaque {st : State} : 
   Code.getReturn (part6_state_update st) = [y0, y1, y2, y3, y4, y5, y6, y7, y8, y9, y10, y11, y12, y13, y14, y15, y16, y17] ↔
-  Code.getReturn (part7_state_update (part6_state st)) = [y0, y1, y2, y3, y4, y5, y6, y7, y8, y9, y10, y11, y12, y13, y14, y15, y16, y17] := by
+  Code.getReturn (part7_state_update (part6_drops (part6_state st))) = [y0, y1, y2, y3, y4, y5, y6, y7, y8, y9, y10, y11, y12, y13, y14, y15, y16, y17] := by
   simp [part6_state_update, part7_wp]
 
 end Risc0.ComputeDecode.Witness.WP
