Risc0/Gadgets/ComputeDecode/Witness/WeakestPreFull.lean
@@ -7,36 +7,38 @@ import Risc0.Gadgets.ComputeDecode.Witness.WeakestPresPart0
 import Risc0.Gadgets.ComputeDecode.Witness.WeakestPresPart1
 import Risc0.Gadgets.ComputeDecode.Witness.WeakestPresPart2
 import Risc0.Gadgets.ComputeDecode.Witness.WeakestPresPart3
--- import Risc0.Gadgets.ComputeDecode.Witness.WeakestPresPart4
--- import Risc0.Gadgets.ComputeDecode.Witness.WeakestPresPart5
--- import Risc0.Gadgets.ComputeDecode.Witness.WeakestPresPart6
--- import Risc0.Gadgets.ComputeDecode.Witness.WeakestPresPart7
--- import Risc0.Gadgets.ComputeDecode.Witness.WeakestPresPart8
--- import Risc0.Gadgets.ComputeDecode.Witness.WeakestPresPart9
--- import Risc0.Gadgets.ComputeDecode.Witness.WeakestPresPart10
--- import Risc0.Gadgets.ComputeDecode.Witness.WeakestPresPart11
--- import Risc0.Gadgets.ComputeDecode.Witness.WeakestPresPart12
--- import Risc0.Gadgets.ComputeDecode.Witness.WeakestPresPart13
--- import Risc0.Gadgets.ComputeDecode.Witness.WeakestPresPart14
--- import Risc0.Gadgets.ComputeDecode.Witness.WeakestPresPart15
--- import Risc0.Gadgets.ComputeDecode.Witness.WeakestPresPart16
--- import Risc0.Gadgets.ComputeDecode.Witness.WeakestPresPart17
--- import Risc0.Gadgets.ComputeDecode.Witness.WeakestPresPart18
--- import Risc0.Gadgets.ComputeDecode.Witness.WeakestPresPart19
--- import Risc0.Gadgets.ComputeDecode.Witness.WeakestPresPart20
--- import Risc0.Gadgets.ComputeDecode.Witness.WeakestPresPart21
--- import Risc0.Gadgets.ComputeDecode.Witness.WeakestPresPart22
--- import Risc0.Gadgets.ComputeDecode.Witness.WeakestPresPart23
--- import Risc0.Gadgets.ComputeDecode.Witness.WeakestPresPart24
--- import Risc0.Gadgets.ComputeDecode.Witness.WeakestPresPart25
--- import Risc0.Gadgets.ComputeDecode.Witness.WeakestPresPart26
--- import Risc0.Gadgets.ComputeDecode.Witness.WeakestPresPart27
--- import Risc0.Gadgets.ComputeDecode.Witness.WeakestPresPart28
--- import Risc0.Gadgets.ComputeDecode.Witness.WeakestPresPart29
--- import Risc0.Gadgets.ComputeDecode.Witness.WeakestPresPart30
--- import Risc0.Gadgets.ComputeDecode.Witness.WeakestPresPart31
+import Risc0.Gadgets.ComputeDecode.Witness.WeakestPresPart4
+import Risc0.Gadgets.ComputeDecode.Witness.WeakestPresPart5
+import Risc0.Gadgets.ComputeDecode.Witness.WeakestPresPart6
+import Risc0.Gadgets.ComputeDecode.Witness.WeakestPresPart7
+import Risc0.Gadgets.ComputeDecode.Witness.WeakestPresPart8
+import Risc0.Gadgets.ComputeDecode.Witness.WeakestPresPart9
+import Risc0.Gadgets.ComputeDecode.Witness.WeakestPresPart10
+import Risc0.Gadgets.ComputeDecode.Witness.WeakestPresPart11
+import Risc0.Gadgets.ComputeDecode.Witness.WeakestPresPart12
+import Risc0.Gadgets.ComputeDecode.Witness.WeakestPresPart13
+import Risc0.Gadgets.ComputeDecode.Witness.WeakestPresPart14
+import Risc0.Gadgets.ComputeDecode.Witness.WeakestPresPart15
+import Risc0.Gadgets.ComputeDecode.Witness.WeakestPresPart16
+import Risc0.Gadgets.ComputeDecode.Witness.WeakestPresPart17
+import Risc0.Gadgets.ComputeDecode.Witness.WeakestPresPart18
+import Risc0.Gadgets.ComputeDecode.Witness.WeakestPresPart19
+import Risc0.Gadgets.ComputeDecode.Witness.WeakestPresPart20
+import Risc0.Gadgets.ComputeDecode.Witness.WeakestPresPart21
+import Risc0.Gadgets.ComputeDecode.Witness.WeakestPresPart22
+import Risc0.Gadgets.ComputeDecode.Witness.WeakestPresPart23
+import Risc0.Gadgets.ComputeDecode.Witness.WeakestPresPart24
+import Risc0.Gadgets.ComputeDecode.Witness.WeakestPresPart25
+import Risc0.Gadgets.ComputeDecode.Witness.WeakestPresPart26
+import Risc0.Gadgets.ComputeDecode.Witness.WeakestPresPart27
+import Risc0.Gadgets.ComputeDecode.Witness.WeakestPresPart28
+import Risc0.Gadgets.ComputeDecode.Witness.WeakestPresPart29
+import Risc0.Gadgets.ComputeDecode.Witness.WeakestPresPart30
+import Risc0.Gadgets.ComputeDecode.Witness.WeakestPresPart31
 
 namespace Risc0.ComputeDecode.Witness.WP
+
+open MLIRNotation
 
 def start_state (input : BufferAtTime) : State :=
   { buffers := Map.fromList [(⟨"in"⟩, [input]), (⟨"data"⟩, [[none, none, none, none, none, none, none, none, none, none, none, none, none, none, none, none, none, none]])]
@@ -49,8 +51,9 @@ def start_state (input : BufferAtTime) : State :=
   , isFailed := false
   }
 
-lemma closed_form {x₀ x₁ x₂ x₃: Felt} {y₀ y₁ y₂ y₃ y₄ y₅ y₆ y₇ y₈ y₉ y₁₀ y₁₁ y₁₂ y₁₃ y₁₄ y₁₅ y₁₆ y₁₇ : Option Felt} :
-  Code.run (start_state [x₀, x₁, x₂, x₃]) = [y₀, y₁, y₂, y₃, y₄, y₅, y₆, y₇, y₈, y₉, y₁₀, y₁₁, y₁₂, y₁₃, y₁₄, y₁₅, y₁₆, y₁₇ ] ↔ sorry := by
+lemma use_opt_full {x₀ x₁ x₂ x₃: Felt} :
+  Code.run (start_state [x₀, x₁, x₂, x₃]) = 
+  Code.getReturn (Γ (start_state [x₀, x₁, x₂, x₃]) ⟦Code.part0; Code.part1; dropfelt ⟨"%74"⟩; dropfelt ⟨"%75"⟩; Code.part2; dropfelt ⟨"%76"⟩; dropfelt ⟨"%77"⟩; Code.part3; dropfelt ⟨"%78"⟩; dropfelt ⟨"%79"⟩; Code.part4; dropfelt ⟨"%80"⟩; dropfelt ⟨"%12"⟩; Code.part5; dropfelt ⟨"%81"⟩; dropfelt ⟨"%10"⟩; Code.part6; dropfelt ⟨"%82"⟩; dropfelt ⟨"%9"⟩; dropfelt ⟨"%83"⟩; dropfelt ⟨"%8"⟩; Code.part7; dropfelt ⟨"%84"⟩; dropfelt ⟨"%85"⟩; Code.part8; dropfelt ⟨"%17"⟩; dropfelt ⟨"%16"⟩; dropfelt ⟨"%86"⟩; dropfelt ⟨"%87"⟩; dropfelt ⟨"%88"⟩; Code.part9; dropfelt ⟨"%89"⟩; dropfelt ⟨"%90"⟩; Code.part10; dropfelt ⟨"%91"⟩; dropfelt ⟨"%92"⟩; Code.part11; dropfelt ⟨"%93"⟩; Code.part12; dropfelt ⟨"%94"⟩; dropfelt ⟨"%95"⟩; Code.part13; dropfelt ⟨"%96"⟩; dropfelt ⟨"%2"⟩; dropfelt ⟨"%97"⟩; Code.part14; dropfelt ⟨"%14"⟩; dropfelt ⟨"%1"⟩; dropfelt ⟨"%98"⟩; dropfelt ⟨"%99"⟩; Code.part15; dropfelt ⟨"%6"⟩; dropfelt ⟨"%5"⟩; dropfelt ⟨"%4"⟩; dropfelt ⟨"%100"⟩; dropfelt ⟨"%101"⟩; Code.part16; dropfelt ⟨"%18"⟩; dropfelt ⟨"%102"⟩; dropfelt ⟨"%103"⟩; Code.part17; dropfelt ⟨"%104"⟩; dropfelt ⟨"%0"⟩; dropfelt ⟨"%105"⟩; Code.part18; dropfelt ⟨"%26"⟩; Code.part19; dropfelt ⟨"%28"⟩; dropfelt ⟨"%29"⟩; dropfelt ⟨"%30"⟩; dropfelt ⟨"%31"⟩; Code.part20; dropfelt ⟨"%27"⟩; dropfelt ⟨"%32"⟩; dropfelt ⟨"%33"⟩; dropfelt ⟨"%25"⟩; Code.part21; dropfelt ⟨"%3"⟩; dropfelt ⟨"%34"⟩; dropfelt ⟨"%35"⟩; dropfelt ⟨"%36"⟩; dropfelt ⟨"%37"⟩; Code.part22; dropfelt ⟨"%23"⟩; dropfelt ⟨"%38"⟩; dropfelt ⟨"%24"⟩; dropfelt ⟨"%39"⟩; dropfelt ⟨"%40"⟩; Code.part23; dropfelt ⟨"%11"⟩; dropfelt ⟨"%42"⟩; dropfelt ⟨"%45"⟩; Code.part24; dropfelt ⟨"%13"⟩; dropfelt ⟨"%46"⟩; dropfelt ⟨"%47"⟩; dropfelt ⟨"%48"⟩; Code.part25; dropfelt ⟨"%43"⟩; dropfelt ⟨"%49"⟩; dropfelt ⟨"%44"⟩; dropfelt ⟨"%50"⟩; dropfelt ⟨"%51"⟩; Code.part26; dropfelt ⟨"%22"⟩; dropfelt ⟨"%52"⟩; dropfelt ⟨"%41"⟩; dropfelt ⟨"%53"⟩; dropfelt ⟨"%54"⟩; Code.part27; dropfelt ⟨"%7"⟩; dropfelt ⟨"%56"⟩; dropfelt ⟨"%59"⟩; Code.part28; dropfelt ⟨"%15"⟩; dropfelt ⟨"%60"⟩; dropfelt ⟨"%58"⟩; dropfelt ⟨"%61"⟩; dropfelt ⟨"%63"⟩; Code.part29; dropfelt ⟨"%57"⟩; dropfelt ⟨"%62"⟩; dropfelt ⟨"%64"⟩; dropfelt ⟨"%65"⟩; dropfelt ⟨"%66"⟩; dropfelt ⟨"%55"⟩; Code.part30; dropfelt ⟨"%19"⟩; dropfelt ⟨"%21"⟩; dropfelt ⟨"%67"⟩; dropfelt ⟨"%68"⟩; dropfelt ⟨"%70"⟩; Code.part31; dropfelt ⟨"%20"⟩; dropfelt ⟨"%71"⟩; dropfelt ⟨"%69"⟩; dropfelt ⟨"%72"⟩; dropfelt ⟨"%73"⟩⟧) := by
   unfold Code.run
   rewrite [Code.optimised_behaviour1]
   rewrite [Code.optimised_behaviour2]
@@ -84,102 +87,111 @@ lemma closed_form {x₀ x₁ x₂ x₃: Felt} {y₀ y₁ y₂ y₃ y₄ y₅ y�
   rewrite [Code.optimised_behaviour30]
   rewrite [Code.optimised_behaviour31]
   rewrite [Code.optimised_behaviour32]
+  rewrite [←Code.opt_full_def]
   unfold MLIR.runProgram
   rewrite [←Code.parts_combine]
   unfold Code.parts_combined
   rewrite [←Code.getReturn_ignores_drops]
-  rewrite [←Code.behaviour_with_drops]
-  rewrite [part0_wp]
-  rewrite [part1_updates_opaque]
-  unfold start_state part0_state
-  MLIR_states_updates
+  rw [←Code.behaviour_with_drops]
 
-  rewrite [part2_updates_opaque]
-  unfold part1_state
-  MLIR_states_updates
-  unfold part1_drops
-  simp [State.dropFelts]
-  MLIR_states_updates
-  simp only [Map.drop_base, ne_eq, Map.update_drop_swap, Map.update_drop]
-  rewrite [Map.drop_of_updates]
-  simp only [Map.drop_base, ne_eq, Map.update_drop_swap, Map.update_drop]
+lemma closed_form {x₀ x₁ x₂ x₃: Felt} {y₀ y₁ y₂ y₃ y₄ y₅ y₆ y₇ y₈ y₉ y₁₀ y₁₁ y₁₂ y₁₃ y₁₄ y₁₅ y₁₆ y₁₇ : Option Felt} :
+  Code.run (start_state [x₀, x₁, x₂, x₃]) = [y₀, y₁, y₂, y₃, y₄, y₅, y₆, y₇, y₈, y₉, y₁₀, y₁₁, y₁₂, y₁₃, y₁₄, y₁₅, y₁₆, y₁₇ ] ↔ sorry := by
+    rewrite [use_opt_full]
+    
+--   rewrite [part0_wp]
+--   rewrite [part1_updates_opaque]
+--   unfold start_state part0_state
+--   MLIR_states_updates
+--   unfold part0_drops
+--   -- no drops
+--   -- no sets
 
-  rewrite [part3_updates_opaque]
-  unfold part2_state
-  MLIR_states_updates
-  unfold part2_drops
-  simp [State.dropFelts]
-  MLIR_states_updates
-  simp only [ne_eq, Map.update_drop_swap, Map.update_drop, Map.drop_base]
-  rewrite [Map.drop_of_updates]
-  simp only [Map.drop_base, ne_eq, Map.update_drop_swap, Map.update_drop]
+--   rewrite [part2_updates_opaque]
+--   unfold part1_state
+--   MLIR_states_updates
+--   unfold part1_drops
+--   simp [State.dropFelts]
+--   MLIR_states_updates
+--   simp only [Map.drop_base, ne_eq, Map.update_drop_swap, Map.update_drop]
+--   rewrite [Map.drop_of_updates]
+--   simp only [Map.drop_base, ne_eq, Map.update_drop_swap, Map.update_drop]
+
+--   rewrite [part3_updates_opaque]
+--   unfold part2_state
+--   MLIR_states_updates
+--   unfold part2_drops
+--   simp [State.dropFelts]
+--   MLIR_states_updates
+--   simp only [ne_eq, Map.update_drop_swap, Map.update_drop, Map.drop_base]
+--   rewrite [Map.drop_of_updates]
+--   simp only [Map.drop_base, ne_eq, Map.update_drop_swap, Map.update_drop]
   
 
-  -- Code.run (start_state [x₀, x₁, x₂, x₃]) = [y₀, y₁, y₂, y₃, y₄, y₅, y₆, y₇, y₈, y₉, y₁₀, y₁₁, y₁₂, y₁₃, y₁₄, y₁₅, y₁₆, y₁₇ ] ↔ sorry := by
-  -- rewrite [part0_wp]
-  -- rewrite [part1_updates_opaque]
-  -- unfold start_state
-  -- unfold part0_state
-  -- MLIR_states_updates
+--   -- Code.run (start_state [x₀, x₁, x₂, x₃]) = [y₀, y₁, y₂, y₃, y₄, y₅, y₆, y₇, y₈, y₉, y₁₀, y₁₁, y₁₂, y₁₃, y₁₄, y₁₅, y₁₆, y₁₇ ] ↔ sorry := by
+--   -- rewrite [part0_wp]
+--   -- rewrite [part1_updates_opaque]
+--   -- unfold start_state
+--   -- unfold part0_state
+--   -- MLIR_states_updates
 
-  -- rewrite [part2_updates_opaque]
-  -- unfold part1_state
-  -- MLIR_states_updates
+--   -- rewrite [part2_updates_opaque]
+--   -- unfold part1_state
+--   -- MLIR_states_updates
 
-  -- rewrite [part3_updates_opaque]
-  -- unfold part2_state
-  -- MLIR_states_updates
+--   -- rewrite [part3_updates_opaque]
+--   -- unfold part2_state
+--   -- MLIR_states_updates
 
-  -- rewrite [part4_updates_opaque]
-  -- unfold part3_state
-  -- MLIR_states_updates
+--   -- rewrite [part4_updates_opaque]
+--   -- unfold part3_state
+--   -- MLIR_states_updates
 
-  -- rewrite [part5_updates_opaque]
-  -- unfold part4_state
-  -- MLIR_states_updates
+--   -- rewrite [part5_updates_opaque]
+--   -- unfold part4_state
+--   -- MLIR_states_updates
 
-  -- rewrite [part6_updates_opaque]
-  -- unfold part5_state
-  -- MLIR_states_updates
+--   -- rewrite [part6_updates_opaque]
+--   -- unfold part5_state
+--   -- MLIR_states_updates
 
-  -- rewrite [part7_updates_opaque]
-  -- unfold part6_state
-  -- MLIR_states_updates
-
-
-  -- generalize h_none : [none, none, none, none, none, none, none, none, none, none, none, none, none, none, none, none, none, none] = nones
-
-  -- -- rewrite [part8_updates_opaque]
-  -- -- unfold part7_state
-  -- -- MLIR_witness_updates
-
-  -- -- rewrite [part9_updates_opaque]
-  -- -- unfold part8_state
-  -- -- MLIR_witness_updates
-
-  -- -- rewrite [part₃_updates_opaque]
-  -- -- rewrite [part₄_updates_opaque]
-  -- -- rewrite [part₅_updates_opaque]
+--   -- rewrite [part7_updates_opaque]
+--   -- unfold part6_state
+--   -- MLIR_states_updates
 
 
+--   -- generalize h_none : [none, none, none, none, none, none, none, none, none, none, none, none, none, none, none, none, none, none] = nones
 
-  -- -- unfold part₁_state
-  -- -- MLIR_witness_updates
+--   -- -- rewrite [part8_updates_opaque]
+--   -- -- unfold part7_state
+--   -- -- MLIR_witness_updates
 
-  -- -- unfold part₂_state
-  -- -- MLIR_witness_updates
+--   -- -- rewrite [part9_updates_opaque]
+--   -- -- unfold part8_state
+--   -- -- MLIR_witness_updates
 
-  -- -- unfold part₃_state
-  -- -- MLIR_witness_updates
+--   -- -- rewrite [part₃_updates_opaque]
+--   -- -- rewrite [part₄_updates_opaque]
+--   -- -- rewrite [part₅_updates_opaque]
 
-  -- -- unfold part₄_state
-  -- -- MLIR_witness_updates
 
-  -- -- unfold part₅_state
-  -- -- MLIR_witness_updates
 
-  -- -- simp [State.lastOutput, Option.get!, List.getLast!, List.getLast, State.buffers]
-  -- -- MLIR_witness_updates
-  -- -- simp [List.getLast]
+--   -- -- unfold part₁_state
+--   -- -- MLIR_witness_updates
+
+--   -- -- unfold part₂_state
+--   -- -- MLIR_witness_updates
+
+--   -- -- unfold part₃_state
+--   -- -- MLIR_witness_updates
+
+--   -- -- unfold part₄_state
+--   -- -- MLIR_witness_updates
+
+--   -- -- unfold part₅_state
+--   -- -- MLIR_witness_updates
+
+--   -- -- simp [State.lastOutput, Option.get!, List.getLast!, List.getLast, State.buffers]
+--   -- -- MLIR_witness_updates
+--   -- -- simp [List.getLast]
 
 end Risc0.ComputeDecode.Witness.WP
